simulations/ctxrefine/MainAdequacy.v
@@ -12,11 +12,11 @@ Require Import ModSim ModSimFacts.
 Require Import HPSim HPSimFacts.
 
 Require Import HMod Mod HMod2Mod Events.
+Require Import SubPerm.
 
-Require Import ISim.
+Require Import ISim ISimFacts.
 Require Import CtxRefine.
-
-Require Import World sWorld.
+Require Import ITactics.
 
 From ExtLib Require Import
      Core.RelDec
@@ -25,344 +25,886 @@ From ExtLib Require Import
 
 Set Implicit Arguments.
 
+Section AUX.
 
-(**** TODO: State theorem & lemmas required for proof's transitivity. ****)
-(* To be moved or merged to another file *)
+  Context `{Σ: GRA.t}.
+
+  Lemma sandbox_well_scoped {A}
+        scopes0 scopes1 (itr: itree hmodE A) 
+        (SCP: incl scopes0 scopes1)
+    :
+      HModSem.sandbox scopes1 (HModSem.sandbox scopes0 itr) = HModSem.sandbox scopes0 itr.
+  Proof.
+    apply bisim_is_eq.
+    revert_until Σ. ginit. gcofix CIH. i.
+    ides itr.
+    - rewrite! HModSB.transl_ret. gstep. econs. eauto.
+    - rewrite! HModSB.transl_tau. gstep. econs. gbase. eauto.
+    - rewrite <- bind_trigger. rewrite! HModSB.transl_bind.
+      destruct e.
+      {
+        assert ((@ITree.trigger (@hmodE Σ) X (inl1 a)) = trigger a) by grind.
+        rewrite H.
+        rewrite! HModSB.transl_ag. rewrite! bind_trigger.
+        gstep. econs. i. r. gbase. eauto.
+      }
+      destruct p.
+      {
+        assert ((@ITree.trigger (@hmodE Σ) X (inr1 (inl1 s))) = trigger s) by grind.
+        rewrite H. rewrite! HModSB.transl_sch. rewrite! bind_trigger.
+        gstep. econs. i. r. gbase. eauto.     
+      }
+      destruct s.
+      {
+        assert ((@ITree.trigger (@hmodE Σ) X (inr1 (inr1 (inl1 c)))) = trigger c) by grind.
+        rewrite H. rewrite! HModSB.transl_call. rewrite! bind_trigger.
+        gstep. econs. i. r. gbase. eauto.     
+      }
+      destruct s.
+      {
+        assert ((@ITree.trigger (@hmodE Σ) X (inr1 (inr1 (inr1 (inl1 p))))) = trigger p) by grind.
+        rewrite H. destruct p.
+        - rewrite! HModSB.transl_put. des_ifs.
+          + rewrite HModSB.transl_put. des_ifs. 
+            * rewrite! bind_trigger. gstep. econs. i. r. gbase. eauto.
+            * exfalso. eapply existsb_exists in Heq. des.
+              eapply SCP in Heq. 
+              assert (XEQ:=existsb_exists).
+              hdes. rewrite XEQ1 in Heq0; ss; eauto.
+          + rewrite HModSB.transl_core.
+            rewrite! bind_trigger. gstep. econs. i. r. gbase. eauto.
+        - rewrite! HModSB.transl_get. des_ifs.
+          + rewrite! HModSB.transl_get. des_ifs.
+            * rewrite! bind_trigger. gstep. econs. i. r. gbase. eauto.
+            * exfalso. eapply existsb_exists in Heq. des.
+              eapply SCP in Heq. 
+              assert (XEQ:=existsb_exists).
+              hdes. rewrite XEQ1 in Heq0; ss; eauto.
+          + rewrite HModSB.transl_core.
+            rewrite! bind_trigger. gstep. econs. i. r. gbase. eauto.
+      }
+      assert ((@ITree.trigger (@hmodE Σ) X (inr1 (inr1 (inr1 (inr1 c))))) = trigger c) by grind.
+      rewrite H. rewrite! HModSB.transl_core. rewrite! bind_trigger.
+      gstep. econs. i. r. gbase. eauto.
+  Qed.
+
+  Lemma inv_sandbox_tau {X}
+        scp (itr: itree hmodE X)
+        (SB: HModSem.sandbox scp (tau;; itr) = tau;; itr)
+      :
+        HModSem.sandbox scp itr = itr.
+  Proof.
+    rewrite HModSB.transl_tau in SB. inv SB.
+    rewrite sandbox_well_scoped; refl.
+  Qed.
+
+  Lemma inv_sandbox_core {X Y}
+        x scp (ktr: X -> itree hmodE Y) (c: coreE X)
+        (SB: HModSem.sandbox scp (trigger c >>= ktr) = trigger c >>= ktr)
+      :
+        HModSem.sandbox scp (ktr x) = ktr x.
+  Proof.
+    rewrite/__ HModSB.transl_bind HModSB.transl_core in SB.
+    rewrite! bind_trigger in SB. inv SB.
+    eapply inj_pair2, equal_f in H0. eauto.
+  Qed.
+
+  Lemma inv_sandbox_call {X Y}
+        x scp (ktr: X -> itree hmodE Y) (c: callE X)
+        (SB: HModSem.sandbox scp (trigger c >>= ktr) = trigger c >>= ktr)
+      :
+        HModSem.sandbox scp (ktr x) = ktr x.
+  Proof.
+    destruct c.
+    rewrite/__ HModSB.transl_bind HModSB.transl_call in SB.
+    rewrite! bind_trigger in SB. inv SB.
+    eapply inj_pair2, equal_f in H0. eauto.
+  Qed.
+
+  Lemma inv_sandbox_pg {X Y}
+        x scp (ktr: X -> itree hmodE Y) (pg: pgE X)
+        (SB: HModSem.sandbox scp (trigger pg >>= ktr) = trigger pg >>= ktr)
+      :
+        HModSem.sandbox scp (ktr x) = ktr x.
+  Proof.
+    destruct pg.
+    { 
+      rewrite/__ HModSB.transl_bind HModSB.transl_put in SB.
+      des_ifs; rewrite! bind_trigger in SB; inv SB.
+      eapply inj_pair2, equal_f in H0. eauto.
+    }
+    { 
+      rewrite/__ HModSB.transl_bind HModSB.transl_get in SB.
+      des_ifs; rewrite! bind_trigger in SB; inv SB.
+      eapply inj_pair2, equal_f in H0. eauto.
+    }
+  Qed.
+  Lemma inv_sandbox_ag {X}
+        scp (ktr: unit -> itree hmodE X) (ag: agE unit)
+        (SB: HModSem.sandbox scp (trigger ag >>= ktr) = trigger ag >>= ktr)
+      :
+        HModSem.sandbox scp (ktr tt) = ktr tt.
+  Proof.
+    rewrite/__ HModSB.transl_bind HModSB.transl_ag in SB.
+    rewrite! bind_trigger in SB. inv SB.
+    eapply inj_pair2, equal_f in H0. eauto.
+  Qed.    
+
+  Lemma alist_upd_fst_in {V} a (k: key) (v: V) l
+    (IN: In a (map (fst <*> fst) l))
+    :
+    In a (map (fst <*> fst) (alist_upd k v l)).
+  Proof.
+    unfold alist_upd in *.
+    induction l; ss; i; rewrite eq_rel_dec_correct; des_ifs; ss; des; eauto.
+  Qed.
+
+  Lemma alist_upd_not_tail {K} `{Dec K} {V} (l1 l2: alist K V) (k: K) (v: V)
+    (NODUP: ¬In k (List.map fst l2))
+    :
+    alist_upd k v (l1 ++ l2) = alist_upd k v l1 ++ l2.
+  Proof.
+    unfold alist_upd.
+    induction l1; ss; cycle 1.
+    {
+      destruct a. ss. rewrite eq_rel_dec_correct. des_ifs; s.
+      rewrite IHl1; eauto.
+    }
+    induction l2; ss.
+    destruct a. ss. rewrite eq_rel_dec_correct. des_ifs; s.
+    { exfalso. eapply not_or_and in NODUP. des. ss. }
+    rewrite IHl2; eauto.
+  Qed.
+
+  Lemma alist_upd_not_in {K V} `{Dec K} (k: K) (v: V) l
+        (NOTIN: ¬ In k (map fst l))
+      :
+        alist_upd k v l = l.
+  Proof.
+    induction l; ss. eapply not_or_and in NOTIN. des.
+    unfold alist_upd. ss. des_ifs.
+    { rewrite eq_rel_dec_correct in Heq. des_ifs. }
+    f_equal. eauto.
+  Qed.
+
+  Lemma alist_upd_not_exists
+        k v st scopes
+        (NOTEXT: existsb (String.eqb k.1) scopes = false)
+        (INSCP: incl (state_scopes st) scopes) 
+      :
+        alist_upd k v st = st.
+  Proof.
+    eapply alist_upd_not_in. 
+    ii. eapply in_map with (f:=fst) in H. 
+    rewrite map_map in H. eapply INSCP in H.
+    assert (∃x, In x scopes /\ String.eqb k.1 x = true).
+    { exists k.1. esplits; [eauto|]. eapply String.eqb_refl. }
+    eapply existsb_exists in H0. clarify.
+  Qed.
+
+  Lemma alist_find_existsb
+        st scopes k v 
+        (INSCP: incl (state_scopes st) scopes) 
+        (FIND: alist_find k st = Some v)
+      :
+        existsb (String.eqb k.1) scopes = true.
+  Proof.
+    eapply existsb_exists.
+    eapply alist_find_fst_some, in_map in FIND.
+    rewrite map_map in FIND.
+    exists k.1. esplits; eauto. eapply String.eqb_refl.
+  Qed.
+
+  Lemma alist_find_not_exists
+        st scopes k
+        (INSCP: incl (state_scopes st) scopes) 
+        (NOTEXT: existsb (String.eqb k.1) scopes = false)
+      :
+        alist_find k st = None.
+  Proof.
+    eapply alist_find_fst_notin.
+    ii. eapply in_map with (f:=fst) in H. 
+    rewrite map_map in H. eapply INSCP in H.
+    assert (∃x, In x scopes /\ String.eqb k.1 x = true).
+    { exists k.1. esplits; [eauto|]. eapply String.eqb_refl. }
+    eapply existsb_exists in H0. clarify.
+  Qed.
+
+  Lemma alist_find_exists_l
+        st ctx scopeS scopeC (k: key)
+        (DISJ: NoDup (scopeS ++ scopeC))
+        (INS: incl (state_scopes st) scopeS)
+        (INC: incl (state_scopes ctx) scopeC)
+        (EXT: existsb (String.eqb k.1) scopeS = true)
+      :
+        alist_find k (st ++ ctx) = alist_find k st.
+  Proof.
+    rewrite alist_find_app_o. des_ifs.
+    eapply alist_find_fst_notin. ii.
+    eapply existsb_exists in EXT. des.
+    eapply NoDup_app_disjoint; eauto.
+    eapply INC. unfold state_scopes. rewrite <- map_map. 
+    eapply in_map with (f:=fst) in H.
+    eapply String.eqb_eq in EXT0. subst. eauto.
+  Qed.
+
+  Lemma wf_eq_solve (a b: Σ) :
+    URA.wf a -> a = b -> URA.wf b.
+  Proof.
+    i. rewrite <- H0. eauto.
+  Qed.
+
+  Lemma wf_inv_l ms0 ms1
+        (WF: HModSem.wf (HModSem.add ms0 ms1))
+      :
+        HModSem.wf ms0.
+  Proof.
+    inv WF; ss. rewrite map_app in wf_fns. 
+    econs; eauto using nodup_app_l.
+  Qed.
+
+  Lemma sk_equiv_ctx sk0 sk1 ctx
+    (EQV: Sk.equiv sk0 sk1)
+  :
+    Sk.equiv (Sk.add sk0 ctx) (Sk.add sk1 ctx).
+  Proof.
+    eapply Permutation_app_tail. eauto.
+  Qed.
+
+End AUX.
+
+
+Section AUX.
+  Context `{Σ: GRA.t}.
+
+  Ltac hstep := guclo hpsimC_spec; econs; econs; eauto; econs; eauto.
+
+  Lemma hpsim_ctx
+    fnsems_src fnsems_tgt fl_src fl_tgt fl_ctx Ist my_tid
+    scopes scopeC
+    (FLS: fl_src = (List.map (map_snd HModSem.sandbox_body) fnsems_src))
+    (FLT: fl_tgt = (List.map (map_snd HModSem.sandbox_body) fnsems_tgt))
+    (WS: ∀ (fn: gname) p (IN: alist_find fn fnsems_src = Some p), incl p.1 scopes)
+    (WT: ∀ (fn: gname) p (IN: alist_find fn fnsems_tgt = Some p), incl p.1 scopes)
+    (DISJ: List.NoDup (scopes ++ scopeC))
+
+    ps pt nths st_src st_tgt st_ctx itr_src itr_tgt fmr
+    (SCPS: incl (state_scopes st_src) scopes)
+    (SCPT: incl (state_scopes st_tgt) scopes)
+    (SCPC: incl (state_scopes st_ctx) scopeC)
+    (ITRS: HModSem.sandbox scopes itr_src = itr_src)
+    (ITRT: HModSem.sandbox scopes itr_tgt = itr_tgt)
+    (SIM: hpsim_body fl_src fl_tgt Ist my_tid ps pt nths (st_src, itr_src) (st_tgt, itr_tgt) fmr)
+    :
+    hpsim_body (fl_src ++ fl_ctx) (fl_tgt ++ fl_ctx) 
+    (IstProd0 (IstSB0 scopes Ist) (IstSB0 scopeC IstEq0)) my_tid
+    ps pt nths (st_src ++ st_ctx, itr_src) (st_tgt ++ st_ctx, itr_tgt) fmr.
+  Proof.
+    guardH FLS. guardH FLT.
+    ginit. s. revert_until DISJ. gcofix CIH. i.
+    exploit SIM; s; i.
+    { eapply nodup_app_l. rewrite <- map_app. eauto. }
+    { eapply nodup_app_l. rewrite <- map_app. eauto. }
+    { subst. eapply nodup_app_l. rewrite <- map_app. eauto. }
+    { subst. eapply nodup_app_l. rewrite <- map_app. eauto. }
+    clear SIM. rename x0 into SIM.
+    remember (st_src, itr_src). remember (st_tgt, itr_tgt).
+    move SIM before CIH. revert_until SIM. punfold SIM.
+    pattern ps, pt, nths, p, p0, fmr.
+    eapply _hpsim_tarski, SIM; i. clear SIM fmr. rename fmr0 into fmr.
+    guclo hpsim_wfC_spec. econs. i. 
+    exploit IN; i; des; eauto. clear IN.
+    destruct x0; i; des; inv Heqp; try inv Heqp0.
+    - hstep. iIntros "H". iPoseProof (RET with "H") as ">[% H]".
+      iModIntro. iSplit; eauto. iExists st_src, st_tgt, st_ctx, st_ctx.
+      iSplit; eauto. iFrame. eauto.
+    - hstep.
+      { 
+        instantiate (1:= FR). iIntros "H". iPoseProof (INV with "H") as ">[H FR]".
+        iModIntro. iFrame. iExists st_src, st_tgt, st_ctx, st_ctx.
+        iSplit; eauto. iFrame. eauto.
+      }
+      i. guclo hpsim_wfC_spec. econs. i.
+      eapply iProp_sepconj_upd in INV0. des.
+      uiprop in INV1. exploit (INV1 rp).
+      { eapply own_wf in INV0; eauto. eapply URA.wf_mon. eauto. }
+      { refl. }
+      clear INV1. intros INV1.
+      unfold IstProd, IstProd0 in INV1.
+      uiprop in INV1. 
+      repeat (rr in INV1; unseal "iProp"; des). ss. des. subst. 
+      repeat (rr in INV3; unseal "iProp"; des). ss. des. subst.
+      repeat (rr in INV6; unseal "iProp"; des). ss. des. subst.
+      repeat (rr in INV1; unseal "iProp"; des). ss. des. subst.
+      repeat (rr in INV3; unseal "iProp"; des). ss. des. subst.
+
+      eapply iProp_Own in INV5.
+      (* 
+        new states after call should maintain the scope of previous states. 
+        ctx state should maintain its own scope.
+      *)
+      eapply K; try refl; eauto using inv_sandbox_call; cycle 3.
+      {
+        uiprop in INV5. exploit (INV5 a0); try refl.
+        { 
+          eapply URA.wf_mon with (b:= a ⋅ a1 ⋅ b ⋅ rq). 
+          eapply own_wf in INV0; eauto.
+          eapply wf_eq_solve; [eapply INV0|r_solve].
+        }
+        clear INV5. intros INV5.
+        repeat (rr in INV5; unseal "iProp"; des). ss. des. subst.
+        rr in INV3; unseal "iProp"; des. ss. 
+      }
+      {
+        uiprop in INV5. exploit (INV5 a0); try refl.
+        { 
+          eapply URA.wf_mon with (b:= a ⋅ a1 ⋅ b ⋅ rq). 
+          eapply own_wf in INV0; eauto.
+          eapply wf_eq_solve; [eapply INV0|r_solve].
+        }
+        clear INV5. intros INV5.
+        repeat (rr in INV5; unseal "iProp"; des). ss. des. subst.
+        rr in INV3; unseal "iProp"; des. ss. 
+      }
+      { eapply nodup_app_l. rewrite <- map_app. eauto. }
+      { eapply nodup_app_l. rewrite <- map_app. eauto. }
+      iIntros "H". iPoseProof (INV0 with "H") as ">H".
+      iDestruct "H" as "[[_ [A _]] Q]".
+      iPoseProof (INV2 with "Q") as "FR".
+      iPoseProof (INV5 with "A") as "(% & IST)".
+      iFrame; eauto.
+    - hstep. i. eapply K; try refl; eauto using inv_sandbox_core. 
+    - hstep. { rewrite alist_find_app_o. rewrite FUN. eauto. }
+      eapply K; try refl; eauto. grind.
+      rewrite! HModSB.transl_bind.
+      move FLS at bottom. move FUN at bottom.
+      rewrite FLS in FUN.
+      rewrite alist_find_map_snd in FUN.
+      unfold o_map in FUN. des_ifs.
+      unfold HModSem.sandbox_body.
+      rewrite sandbox_well_scoped; eauto.
+      f_equal. extensionalities.
+      rewrite/__ !HModSB.transl_bind !HModSB.transl_ret.
+      f_equal. extensionalities. eapply inv_sandbox_call; eauto. 
+
+    - hstep. { rewrite alist_find_app_o. rewrite FUN. eauto. }
+      eapply K; try refl; eauto. grind.
+      rewrite! HModSB.transl_bind.
+      move FLT at bottom. move FUN at bottom.
+      rewrite FLT in FUN.
+      rewrite alist_find_map_snd in FUN.
+      unfold o_map in FUN. des_ifs.
+      unfold HModSem.sandbox_body.
+      rewrite sandbox_well_scoped; eauto.
+      f_equal. extensionalities.
+      rewrite/__ !HModSB.transl_bind !HModSB.transl_ret.
+      f_equal. extensionalities. eapply inv_sandbox_call; eauto. 
+    - hstep. eapply K; try refl; eauto using inv_sandbox_tau.
+    - hstep. eapply K; try refl; eauto using inv_sandbox_tau.
+    - hstep. i. eapply K; try refl; eauto using inv_sandbox_core.
+    - hstep. i. eapply K; try refl; eauto using inv_sandbox_core.
+    - hstep. eapply K; try refl; eauto using inv_sandbox_core.
+    - hstep. eapply K; try refl; eauto using inv_sandbox_core.
+    - assert (H1:= ITRS).
+      rewrite /__ -ITRS HModSB.transl_bind HModSB.transl_put. des_ifs.
+      + hstep.
+        assert (UPD: alist_upd k v (st_src ++ st_ctx) = alist_upd k v st_src ++ st_ctx).
+        { 
+          move SCPS at bottom. move SCPC at bottom. 
+          eapply existsb_exists in Heq. des. eapply String.eqb_eq in Heq0.
+          rewrite alist_upd_not_tail; eauto.
+          ii. eapply NoDup_app_disjoint; eauto.
+          eapply in_map with (f:=fst) in H2.
+          rewrite map_map in H2. eapply SCPC in H2.
+          rewrite <- Heq0. eauto.
+        }
+        rewrite UPD. eapply K; try refl; eauto.
+        { rewrite state_scopes_update. eauto. }
+        { eapply sandbox_well_scoped. refl. }
+        { rewrite <-UPD. eapply alist_upd_nodup. eauto. }
+        { f_equal. symmetry. eapply inv_sandbox_pg. eauto. }
+      + hstep. eapply K; try refl; eauto.
+        { eapply sandbox_well_scoped. refl. }
+        { 
+          f_equal. 
+          { eapply alist_upd_not_exists; eauto. }
+          { symmetry. eapply inv_sandbox_pg. eauto. }
+        }
+
+    - assert (H1:=ITRT).
+      rewrite/__ -ITRT HModSB.transl_bind HModSB.transl_put. des_ifs.
+      + hstep.
+        assert (UPD: alist_upd k v (st_tgt ++ st_ctx) = alist_upd k v st_tgt ++ st_ctx).
+        {
+          move SCPS at bottom. move SCPC at bottom. 
+          eapply existsb_exists in Heq. des. eapply String.eqb_eq in Heq0.
+          eapply alist_upd_not_tail. eauto.
+          ii. eapply NoDup_app_disjoint; eauto.
+          eapply in_map with (f:=fst) in H2.
+          rewrite map_map in H2. eapply SCPC in H2.
+          rewrite <- Heq0. eauto.  
+        }
+        rewrite UPD. eapply K; try refl; eauto.
+        { rewrite state_scopes_update. eauto. }
+        { eapply sandbox_well_scoped. refl. }
+        { rewrite <-UPD. eapply alist_upd_nodup. eauto. }
+        { f_equal. symmetry. eapply inv_sandbox_pg. eauto. }
+      + rewrite/__ HModSB.transl_bind HModSB.transl_put Heq !bind_trigger in H1.
+      exfalso. ss.   
+
+    - assert (H1:=ITRS). 
+      rewrite/__  -ITRS HModSB.transl_bind HModSB.transl_get. des_ifs.
+      + hstep. eapply K; try refl; eauto.
+        { eapply sandbox_well_scoped. refl. }
+        erewrite alist_find_exists_l; eauto.
+        repeat f_equal. symmetry. eapply inv_sandbox_pg; eauto. 
+      + hstep. eapply K; try refl; eauto.
+        { eapply sandbox_well_scoped. refl. }
+        repeat f_equal. symmetry. unfold or_else. 
+        erewrite alist_find_not_exists; eauto.
+        eapply inv_sandbox_pg; eauto.
+
+    - assert (H1:=ITRT). 
+      rewrite/__  -ITRT HModSB.transl_bind HModSB.transl_get. des_ifs.
+      + hstep. eapply K; try refl; eauto.
+        { eapply sandbox_well_scoped. refl. }
+        erewrite alist_find_exists_l; eauto.
+        repeat f_equal. symmetry. eapply inv_sandbox_pg; eauto. 
+      + rewrite/__ HModSB.transl_bind HModSB.transl_get Heq !bind_trigger in H1.
+        exfalso. ss.
+
+    - hstep. i. eapply K; try refl; eauto using inv_sandbox_ag.
+    - hstep. i. eapply K; try refl; eauto using inv_sandbox_ag.
+    - hstep. i. eapply K; try refl; eauto using inv_sandbox_ag.
+    - hstep. i. eapply K; try refl; eauto using inv_sandbox_ag.
+    - hstep. eapply K; try refl; eauto.
+      + rewrite/__ HModSB.transl_bind HModSB.transl_sch !bind_trigger in ITRS.
+        depdes ITRS. eapply equal_f in x. eauto.
+      + rewrite/__ HModSB.transl_bind HModSB.transl_sch !bind_trigger in ITRT.
+        depdes ITRT. eapply equal_f in x. eauto.
+    - hstep.
+      { 
+        instantiate (1:= FR). iIntros "H". iPoseProof (INV with "H") as ">[H FR]".
+        iModIntro. iFrame. iExists st_src, st_tgt, st_ctx, st_ctx.
+        iSplit; eauto. iFrame. eauto.
+      }
+      i. guclo hpsim_wfC_spec. econs. i.
+      eapply iProp_sepconj_upd in INV0. des.
+      uiprop in INV1. exploit (INV1 rp).
+      { eapply own_wf in INV0; eauto. eapply URA.wf_mon. eauto. }
+      { refl. }
+      clear INV1. intros INV1.
+      unfold IstProd, IstProd0 in INV1.
+      uiprop in INV1. 
+      repeat (rr in INV1; unseal "iProp"; des). ss. des. subst. 
+      repeat (rr in INV3; unseal "iProp"; des). ss. des. subst.
+      repeat (rr in INV6; unseal "iProp"; des). ss. des. subst.
+      repeat (rr in INV1; unseal "iProp"; des). ss. des. subst.
+      repeat (rr in INV3; unseal "iProp"; des). ss. des. subst.
+
+      eapply iProp_Own in INV5.
+      (* 
+        new states after call should maintain the scope of previous states. 
+        ctx state should maintain its own scope.
+      *)
+      eapply K; try refl; eauto using inv_sandbox_call; cycle 3.
+      {
+        uiprop in INV5. exploit (INV5 a0); try refl.
+        { 
+          eapply URA.wf_mon with (b:= a ⋅ a1 ⋅ b ⋅ rq). 
+          eapply own_wf in INV0; eauto.
+          eapply wf_eq_solve; [eapply INV0|r_solve].
+        }
+        clear INV5. intros INV5.
+        repeat (rr in INV5; unseal "iProp"; des). ss. des. subst.
+        rr in INV3; unseal "iProp"; des. ss. 
+      }
+      {
+        uiprop in INV5. exploit (INV5 a0); try refl.
+        { 
+          eapply URA.wf_mon with (b:= a ⋅ a1 ⋅ b ⋅ rq). 
+          eapply own_wf in INV0; eauto.
+          eapply wf_eq_solve; [eapply INV0|r_solve].
+        }
+        clear INV5. intros INV5.
+        repeat (rr in INV5; unseal "iProp"; des). ss. des. subst.
+        rr in INV3; unseal "iProp"; des. ss. 
+      }
+      { rewrite/__ HModSB.transl_bind HModSB.transl_sch !bind_trigger in ITRS.
+        depdes ITRS. eapply equal_f in x. eauto. }
+      { rewrite/__ HModSB.transl_bind HModSB.transl_sch !bind_trigger in ITRT.
+        depdes ITRT. eapply equal_f in x. eauto. }
+      { eapply nodup_app_l. rewrite <- map_app. eauto. }
+      { eapply nodup_app_l. rewrite <- map_app. eauto. }
+      iIntros "H". iPoseProof (INV0 with "H") as ">H".
+      iDestruct "H" as "[[_ [A _]] Q]".
+      iPoseProof (INV2 with "Q") as "FR".
+      iPoseProof (INV5 with "A") as "(% & IST)".
+      iFrame; eauto.
+
+    - hstep. eapply K; try refl; eauto.
+      rewrite/__ HModSB.transl_bind HModSB.transl_sch !bind_trigger in ITRS.
+      depdes ITRS. eapply equal_f in x. eauto.
+      
+    - hstep. eapply K; try refl; eauto.
+      rewrite/__ HModSB.transl_bind HModSB.transl_sch !bind_trigger in ITRT.
+      depdes ITRT. eapply equal_f in x. eauto.
+      
+    - gstep. econs. econs. econs; eauto. econs; eauto. 
+      gbase. pclearbot. eapply CIH; try refl; eauto.
+      ii. eauto.
+  Qed.
+
+  Lemma isim_ctx
+    fs ft ms mt ctx Ist fn
+    (WFS: HModSem.wf (HModSem.add ms ctx))
+    (WFT: HModSem.wf (HModSem.add mt ctx))
+    (FINDS: alist_find fn (HModSem.fnsems ms) = Some fs)
+    (FINDT: alist_find fn (HModSem.fnsems mt) = Some ft)
+    (SCOPES: sub_perm (HModSem.scopes mt) (HModSem.scopes ms))
+    (NODUPFS: NoDup (map fst (HModSem.fnsems ms ++ HModSem.fnsems ctx)))
+    (NODUPFT: NoDup (map fst (HModSem.fnsems mt ++ HModSem.fnsems ctx)))
+    (IMON: ∀ nths0 nths', nths0 <= nths' → ∀ st_src st_tgt,
+           Ist nths0 st_src st_tgt -∗ Ist nths' st_src st_tgt)
+    (SIM: isim_fsem
+       (map (map_snd HModSem.sandbox_body) (HModSem.fnsems ms))
+       (map (map_snd HModSem.sandbox_body) (HModSem.fnsems mt))
+       Ist
+       (HModSem.sandbox_body fs)
+       (HModSem.sandbox_body ft))
+    :
+      isim_fsem
+        (map (map_snd HModSem.sandbox_body)
+           (HModSem.fnsems ms ++ HModSem.fnsems ctx))
+        (map (map_snd HModSem.sandbox_body)
+           (HModSem.fnsems mt ++ HModSem.fnsems ctx))
+        (IstProd0 (IstSB0 (HModSem.scopes ms) Ist) (IstSB0 (HModSem.scopes ctx) IstEq0))
+        (HModSem.sandbox_body fs) (HModSem.sandbox_body ft).
+  Proof.
+    ii. specialize (SIM x y H). subst.
+    iIntros "H". iDestruct "H" as (? ? ? ?) "(% & (% & IST) & %)". des. subst.
+    rewrite map_app in *. 
+    assert (NODA := NODS). assert (NODB := NODD). assert (NODC:= NODS).
+    eapply nodup_app_l in NODA, NODB. eapply nodup_app_r in NODC.
+    specialize (SIM my_tid nths st_srcL st_tgtL IMON NODA NODB).
+    rewrite <- map_app in *.
+    iPoseProof (SIM with "IST") as "SIM".
+    iStopProof. Local Transparent isim.
+    uiprop. i.
+    gfinal. right. eapply paco8_mon_bot; eauto.
+    rewrite! List.map_app.
+    assert (EQ: (λ x, (map_snd HModSem.sandbox_body x).1) = @fst string _).
+    { extensionalities. destruct H2. eauto. }
+    eapply hpsim_ctx; eauto; ss; cycle 6.
+    { rewrite/__ -map_app map_map EQ. eauto. }
+    { rewrite/__ -map_app map_map EQ. eauto. }
+    { 
+      ii. eapply ms.(HModSem.well_scoped_fns).
+      unfold fnsems_scopes. rewrite IN. ss.
+    }
+    {
+      i. etrans; cycle 1.
+      { eapply sub_perm_incl; eauto. }
+      ii. eapply mt.(HModSem.well_scoped_fns).
+      unfold fnsems_scopes. rewrite IN. ss.
+    }
+    { eapply WFS. }
+    { 
+      eapply sandbox_well_scoped. ii.
+      eapply ms.(HModSem.well_scoped_fns). 
+      unfold fnsems_scopes. rewrite FINDS. ss.
+    }
+    { 
+      eapply sandbox_well_scoped. etrans; cycle 1.
+      { eapply sub_perm_incl; eauto. }
+      ii. eapply mt.(HModSem.well_scoped_fns). 
+      unfold fnsems_scopes. rewrite FINDT. ss.
+    }
+    ginit. i. eapply gpaco8_mon; eauto using iunlift_ibot.
+  Qed.
+
+  Lemma hmod_sim_ctx (ms mt ctx: HMod.t) IC Ist
+    (SIM: HSim.t ms mt IC Ist)
+    :
+    HSim.t (ms ★ ctx) (mt ★ ctx) IC 
+      (fun sk => IstProd0 (IstSB0 (HMod.modsem ms sk).(HModSem.scopes) (Ist sk))
+                          (IstSB0 (HMod.modsem ctx sk).(HModSem.scopes) IstEq0)).
+  Proof.
+    inv SIM.
+    econs; cycle 1.
+    { ss. r. eapply sk_equiv_ctx. eauto. }
+    i. hexploit sim_modsem; eauto.
+    { 
+      r in SKINCL. ii. hexploit (SKINCL a); eauto.
+      ss. eapply in_or_app; eauto.
+    }
+    i. inv H. econs; ss.
+    { 
+      iIntros "H". iPoseProof (sim_initial with "H") as "H".
+      unfold IstProd. iExists _, _, _, _. iFrame. iPureIntro.
+      esplits; eauto; try eapply HModSem.well_scoped_init.
+      etrans; [eapply HModSem.well_scoped_init|].
+      eapply sub_perm_incl, sim_scopes.
+    }
+    { i. iIntros "H". iDestruct "H" as (? ? ? ?) "(% & (% & H) & %)". des; subst.
+      iPoseProof ((sim_mon _ _ LE) with "H") as "H".
+      repeat iExists _. iFrame. iPureIntro. esplits; eauto.
+    }
+    { eapply sub_perm_cancel_tail. eauto. }
+    { rewrite! app_length. nia. }
+    {
+      i. rewrite map_app in *. eapply in_app_or in IN.
+      des; eapply in_or_app; eauto.  
+    }
+    r. i. ss. rewrite alist_find_app_o in FIND. des_ifs.
+    {
+      (* find in src/tgt module *)
+      hexploit sim_fnsems; i.
+      { eapply alist_find_fst_some. eauto. }
+      r in H. hexploit H; eauto; i.
+      { 
+        inv WFS; ss. econs.  
+        { rewrite map_app in wf_fns. eapply nodup_app_l. eauto. }
+        { eapply nodup_app_l; eauto. }
+      }
+      { 
+        inv WFT; ss. econs.  
+        { rewrite map_app in wf_fns. eapply nodup_app_l. eauto. }
+        { eapply nodup_app_l; eauto. }
+      }
+      { eapply nodup_app_l. rewrite <- map_app. eauto. }
+      { eapply nodup_app_l. rewrite <- map_app. eauto. }
+      des. esplits.
+      { rewrite alist_find_app_o. des_ifs. }
+      eapply isim_ctx; eauto.
+    } 
+    {
+      destruct fs as [scp itr]. esplits; ss.
+      { rewrite alist_find_app_o. des_ifs; eauto.
+        exfalso.
+        eapply alist_find_fst_some, hssim_match, alist_find_fst_in in Heq0.
+        - des. rewrite Heq in Heq0. ss.
+        - econs; eauto.
+        - rewrite map_app in NODUPFS. eapply nodup_app_l. eauto.
+      }
+      inv WFS. eapply isim_reflR; ss; i; eauto.
+      - replace scp with (fnsems_scopes fn (HMod.modsem ctx sk).(HModSem.fnsems)).
+        { eapply (HMod.modsem ctx sk).(HModSem.well_scoped_fns). }
+        { unfold fnsems_scopes. des_ifs. }
+      - iIntros "%". des; subst; eauto.
+      - iIntros "%". des; subst; eauto. iPureIntro.  esplits; eauto.
+        + rewrite state_scopes_update. eauto.
+        + rewrite state_scopes_update. eauto.
+    }
+  Qed.
+
+End AUX.
 
 Section ADEQUACY.
 
   Context `{Σ: GRA.t}.
 
   Theorem main_adequacy (ms mt: HMod.t) IC Ist
-    (SIM: HModR.sim ms mt IC Ist)
+    (SIM: HSim.t ms mt IC Ist)
     :
     ctx_refines (ms,IC) (mt, const(emp%I)).
   Proof.
-  Admitted.
+    ii. s. split.
+    { s. eapply sk_equiv_ctx. apply SIM. }
+
+    destruct ctx as [ctx cond].
+    assert (SIMC := SIM).
+    ii. eapply hmod_sim_ctx with (ctx := ctx) in SIMC.
+    hexploit (HSim.sim_modsem SIMC); eauto.
+    { eapply Sk.equiv_incl in EQV. etrans; eauto. refl. }
+    i. ss.
+
+    eapply iProp_sepconj in SRC; eauto. des.
+    esplits. 
+    { rewrite SRC in WFR. rewrite URA.add_comm in WFR. eapply URA.wf_mon. eauto. }
+    { 
+      eapply iProp_Own in SRC1. iIntros "H".
+      iPoseProof (SRC1 with "H") as "H". iFrame. eauto.
+    }
+    { eapply hssim_wf; eauto. }
+    ii. subst. eapply adequacy_modsem, PR.
+    - eapply hssim_adequacy; eauto.
+      eapply hssim_wf; eauto.
+    - inv WFM. econs. ss. unfold map_snd.
+      rewrite !List.map_map. eapply eq_ind; [apply wf_fns|].
+      f_equal. extensionalities. destruct H0. ss.
+  Qed.
 
 End ADEQUACY.
 
-(*
+Section COMM.
 
-Section ADEQUACY.
-  (* Context `{_W: CtxWD.t}. *)
   Context `{Σ: GRA.t}.
 
-  Lemma Own_upd_specify
-        r P 
-        (UPD: Own r ⊢ #=> P) 
-        (WF: URA.wf r):
-    exists r0, P r0 /\ URA.updatable r r0.
-  Proof.
-    uiprop in UPD. specialize (UPD r WF).
-    hexploit UPD; [refl|]. i. des.
-    esplits; eauto.
-  Qed.
-
-  Theorem adequacy_hmod
-      (md_src md_tgt: HMod.t) Ist
-      (rs rt: Σ) 
-      (* (WF: URA.wf rs) *)
-      (* (SRC: forall sk, 
-        HModSem.initial_cond (md_src.(HMod.get_modsem) sk) rs) *)
-      (* (TGT: forall sk,
-        HModSem.initial_cond (md_tgt.(HMod.get_modsem) sk) rt) *)
-      (SRC: HModSem.initial_cond (md_src.(HMod.get_modsem) md_src.(HMod.sk)) rs)
-      (TGT: HModSem.initial_cond (md_tgt.(HMod.get_modsem) md_tgt.(HMod.sk)) rt)
-      (SIM: HModR.sim md_src md_tgt Ist)
-    :
-      ModR.sim (HMod.to_mod md_src rs) (HMod.to_mod md_tgt rt).
-  Proof.
-    (* inv SIM. des.
-    econs; eauto. i. specialize (sim_modsem sk SKINCL SKWF).
-    specialize (SRC sk). specialize (TGT sk). 
-    des. inv sim_modsem.
-    econs; ss.
-    - instantiate (1:= eq). eapply base.PreOrder_instance_0.
-    - instantiate (1:= interp_inv Ist).
-      exists ε. econs; eauto.
-      {
-        iIntros "H". eapply iProp_Own in SRC. iPoseProof (SRC with "H") as "H".
-        iPoseProof (sim_initial with "H") as "[TGT IST]".
-        admit.
-      }
-      admit.
-    - rewrite! List.map_length. eauto.
-    - i. rewrite alist_find_map in *. unfold o_map in *. des_ifs.
-      eapply sim_miss in Heq0. clarify.
-    - i. rewrite alist_find_map in *. unfold o_map in *. des_ifs; cycle 1.
-      { eapply sim_fnsems in Heq0. des. clarify. }
-      esplits; eauto.
-      ii. subst. inv SIMMRS. eapply hpsim_adequacy; eauto; cycle 1.
-      { r_solve. eauto. }
-      { instantiate (1:= mr). r_solve. eauto. }
-      ginit. apply gpaco7_mon with (r := iunlift ibot) (rg := iunlift ibot); eauto using iunlift_ibot.
-      guclo hpsim_wfC_spec. econs. i.
-      eapply Own_upd_specify in MR; eauto. des.
-      guclo hpsim_updateC_spec. econs. econs. instantiate (1:= r0).
-      esplits; eauto using Own_Upd.
-      eapply isim_init; cycle 1. { eapply iProp_Own. eauto. }
-      hexploit sim_fnsems; eauto. i. des.
-      assert (i = ft). { rewrite Heq in H1. inv H1. eauto. }
-      subst. do 2 r in H2. hexploit (H2 y y); eauto. *)
-      
+  Definition perm_Ist: nat -> alist key Any.t -> alist key Any.t -> iProp :=
+    fun _ l0 l1 => ⌜l0 ≡ₚ l1⌝%I.  
   
-(*     
-    - instantiate (1:= eq). eapply base.PreOrder_instance_0.
-    - ss. unfold cond_to_st, handle_init_cond, assume_init. grind.
-      ginit. 
-      gstep. econs; eauto. i. grind. econs; eauto. i. econs; eauto. i. (* run src to the end *)
-      assert (Own x ⊢ HModSem.initial_cond (HMod.get_modsem md_tgt sk) **
-      Ist (HModSem.initial_st (HMod.get_modsem md_src sk)) (HModSem.initial_st (HMod.get_modsem md_tgt sk))).
-      { iIntros "H". iApply isim_initial. iApply x1. eauto. }
-      eapply iProp_sepconj in H; cycle 1. { eapply URA.wf_mon. eauto. }
-      des.
-      econs; eauto. instantiate (1:= p). grind. econs; eauto. { r_solve. do 2 eapply URA.wf_mon. eauto. } 
-      econs; eauto. { eapply iProp_Own. eauto. }
-      econs. exists (ε: Σ). instantiate (1:= interp_inv Ist). hss. 
-      econs; eauto.
-      { instantiate (1:= q). r_solve. rewrite URA.add_comm. eauto. }
-      eapply iProp_Own in H1. iIntros "H". iApply (H1 with "H").
-    - eapply Forall2_apply_Forall2; eauto.
-      i. destruct a, b. inv H. econs; ss. ii. do 3 r in H1.
-        specialize (H1 x y H). inv SIMMRS. s.
-        specialize (H1 st_src st_tgt).
-        eapply hpsim_adequacy; [et|et| |r_solve;et|]; cycle 1.
-        { instantiate (1:= mr). r_solve. eauto. }
-        ginit. guclo hpsim_wfC_spec. econs. i.
-        eapply Own_upd_specify in MR; eauto. des.
-        eapply Own_Upd in MR0.
-        guclo hpsim_updateC_spec. econs. econs.
-        instantiate (1:= r0). esplits; eauto.
-        eapply iProp_Own in MR. eapply isim_init in H1; eauto.
-        eapply gpaco7_mon; eauto using iunlift_ibot. *)
-
-  Admitted.
-
-  (* Theorem adequacy_hmod
-      (md_src md_tgt: HMod.t) Ist
-      (SIM: HModR.sim md_src md_tgt Ist)
-    :
-      ModR.sim (HMod.to_mod md_src) (HMod.to_mod md_tgt).
+  Lemma alist_upd_perm {K V} l0 l1 `{Dec K} (k: K) (v: V)
+        (ND: NoDup (map fst l0))
+        (PERM: l0 ≡ₚ l1)
+      :
+        alist_upd k v l0 ≡ₚ alist_upd k v l1.
   Proof.
-    inv SIM. des.
-    econs; eauto. i. specialize (sim_modsem sk SKINCL SKWF). 
-    des. inv sim_modsem.
-    econs; swap 2 3.
-    - instantiate (1:= eq). eapply base.PreOrder_instance_0.
-    - ss. unfold cond_to_st, handle_init_cond, assume_init. grind.
-      ginit. 
-      gstep. econs; eauto. i. grind. econs; eauto. i. econs; eauto. i. (* run src to the end *)
-      assert (Own x ⊢ HModSem.initial_cond (HMod.get_modsem md_tgt sk) **
-      Ist (HModSem.initial_st (HMod.get_modsem md_src sk)) (HModSem.initial_st (HMod.get_modsem md_tgt sk))).
-      { iIntros "H". iApply isim_initial. iApply x1. eauto. }
-      eapply iProp_sepconj in H; cycle 1. { eapply URA.wf_mon. eauto. }
-      des.
-      econs; eauto. instantiate (1:= p). grind. econs; eauto. { r_solve. do 2 eapply URA.wf_mon. eauto. } 
-      econs; eauto. { eapply iProp_Own. eauto. }
-      econs. exists (ε: Σ). instantiate (1:= interp_inv Ist). hss. 
-      econs; eauto.
-      { instantiate (1:= q). r_solve. rewrite URA.add_comm. eauto. }
-      eapply iProp_Own in H1. iIntros "H". iApply (H1 with "H").
-    - eapply Forall2_apply_Forall2; eauto.
-      i. destruct a, b. inv H. econs; ss. ii. do 3 r in H1.
-        specialize (H1 x y H). inv SIMMRS. s.
-        specialize (H1 st_src st_tgt).
-        eapply hpsim_adequacy; [et|et| |r_solve;et|]; cycle 1.
-        { instantiate (1:= mr). r_solve. eauto. }
-        ginit. guclo hpsim_wfC_spec. econs. i.
-        eapply Own_upd_specify in MR; eauto. des.
-        eapply Own_Upd in MR0.
-        guclo hpsim_updateC_spec. econs. econs.
-        instantiate (1:= r0). esplits; eauto.
-        eapply iProp_Own in MR. eapply isim_init in H1; eauto.
-        eapply gpaco7_mon; eauto using iunlift_ibot.
-  Qed. *)
-
-End ADEQUACY.
-
-Section HPSIM.
-  Context `{Σ: GRA.t}.
-  Import HModSem.
-
-  Definition addf f1 f2 : alist gname (Any.t -> itree _ Any.t) :=
-    (List.map trans_l f1) ++ (List.map trans_r f2).
-
-  Lemma IstProdEq 
-        Ist stl str stc
-    :
-        Ist stl str
-      -∗
-        IstProd Ist IstEq (Any.pair stl stc) (Any.pair str stc).
-  Proof.
-    iIntros "H". unfold IstProd, IstEq. iExists stl, str, _, _.
-    iFrame. iPureIntro. esplits; eauto.
+    destruct (classic (In k (map fst l0))); cycle 1.
+    {
+      rewrite! alist_upd_not_in; eauto. ii.
+      eapply H0. eapply Permutation_in; cycle 1; eauto.
+      eapply Permutation_map. symmetry. eauto.
+    }
+    assert (NoDup (map fst l1)).
+    { 
+      eapply Permutation_NoDup; cycle 1; eauto. 
+      eapply Permutation_map. eauto.
+    }
+    eapply alist_find_fst_in in H0. des.
+    eapply alist_find_some in H0.
+    assert (In (k, v0) l1).
+    { eapply Permutation_in; eauto. }
+    eapply in_split in H0, H2. des. subst.
+    replace (l4 ++ (k, v0) :: l5) with ((l4 ++ [(k, v0)] ++ l5)); eauto.
+    replace (l2 ++ (k, v0) :: l3) with ((l2 ++ [(k, v0)] ++ l3)); eauto.
+    rewrite! alist_upd_with_nodup; eauto.
+    eapply Permutation_app_middle, Permutation_app_inv. eauto.
+    Unshelve. eauto.
   Qed.
 
-  Ltac hstep := guclo hpsimC_spec; econs; econs; eauto; econs; eauto.
-
-  (* Not necessary if you can prove isim_ctx_aux directly. *)
-  Theorem hpsim_ctx
-          fl_src fl_tgt fl_ctx Ist
-          ps pt st_src st_tgt st_ctx itr_src itr_tgt
-          fmr stl str
-          (SIM: hpsim_body fl_src fl_tgt Ist ps pt (st_src, itr_src) (st_tgt, itr_tgt) fmr)
-          (SRC: stl = Any.pair st_src st_ctx)
-          (TGT: str = Any.pair st_tgt st_ctx)
-      :
-          hpsim_body (addf fl_src fl_ctx) (addf fl_tgt fl_ctx) (IstProd Ist IstEq) 
-          ps pt (stl, translate (emb_ run_l) itr_src) (str, translate (emb_ run_l) itr_tgt) fmr.
+  Lemma alist_permutation_find K `{Dec K} V (l0 l1: alist K V)
+        (ND: List.NoDup (List.map fst l0))
+        (PERM: Permutation l0 l1)
+        k
+    :
+      alist_find k l0 = alist_find k l1.
   Proof.
-    revert_until Σ. ginit. gcofix CIH. i.
-    remember (st_src, itr_src). remember (st_tgt, itr_tgt).
-    move SIM before Σ. revert_until SIM. punfold SIM.
-    pattern ps, pt, p, p0, fmr.
-    eapply _hpsim_tarski, SIM; i. clear SIM fmr. rename fmr0 into fmr.
-    guclo hpsim_wfC_spec. econs. i. 
-    exploit IN; i; des; eauto.
-    destruct x0; i; des; inv Heqp; try inv Heqp0.
-    - rewrite! translate_emb_ret. hstep.
-      iIntros "H". iPoseProof (RET with "H") as ">[H %]".
-      iModIntro. iSplit; eauto. iApply IstProdEq. eauto.
-    - rewrite! translate_emb_bind. rewrite! translate_emb_callE. hstep.
-      { 
-        instantiate (1:= FR). iIntros "H". iPoseProof (INV with "H") as ">[H FR]".
-        iModIntro. iFrame. iApply IstProdEq. eauto.
-      }
-      (* 
-        Property about Any.pair is not restored without Own fmr1. 
-      *)
-      i. guclo hpsim_wfC_spec. econs. i.
- 
-      eapply K; eauto; admit.
-    - rewrite! translate_emb_bind. rewrite! translate_emb_coreE. hstep.
-    - rewrite! translate_emb_bind. rewrite translate_emb_callE. hstep.
-      { unfold addf. apply alist_find_app. unfold trans_l. rewrite alist_find_map. unfold o_map. rewrite FUN. et. }
-      s. (* put Ret ();;; Ret x back into translate () *) admit.
-    - rewrite! translate_emb_bind. admit.
-    - rewrite! translate_emb_tau. hstep.
-    - rewrite! translate_emb_tau. hstep.
-    - rewrite! translate_emb_bind. rewrite! translate_emb_coreE. hstep.
-    - rewrite! translate_emb_bind. rewrite! translate_emb_coreE. hstep.
-    - rewrite! translate_emb_bind. rewrite! translate_emb_coreE. hstep.
-    - rewrite! translate_emb_bind. rewrite! translate_emb_coreE. hstep.
-    - rewrite! translate_emb_bind. rewrite! translate_emb_sE. hstep. hss. des_ifs.
-    - rewrite! translate_emb_bind. rewrite! translate_emb_sE. hstep. hss. des_ifs.
-    - rewrite! translate_emb_bind. rewrite translate_emb_assume. hstep.
-    - rewrite! translate_emb_bind. rewrite translate_emb_guarantee. hstep.
-    - rewrite! translate_emb_bind. rewrite translate_emb_guarantee. hstep.
-    - rewrite! translate_emb_bind. rewrite translate_emb_assume. hstep.
-    - gstep. econs. econs. econs; eauto. econs; eauto. 
-      gbase. pclearbot. eapply CIH; eauto.
-  Admitted.
-
-
-          
-          
-
-End HPSIM.
-
-Section SIM.
-  Context `{Σ: GRA.t}.
-  (* Context `{_W: CtxWD.t}. *)
-  Section HMODSEM.
-    Import HModSem.
-
-    Ltac cq := apply combine_quant.
-
-    Lemma any_pair_inv 
-          a0 a1 b0 b1
-          (PAIR: Any.pair a0 a1 = Any.pair b0 b1)
-        :
-           a0 = b0 /\ a1 = b1.
-    Proof.
-      destruct (Any.split (Any.pair a0 a1)) eqn:E; cycle 1.
-      { rewrite Any.pair_split in E. inv E. }
-      destruct p. hexploit E. i.
-      rewrite PAIR in H. 
-      rewrite Any.pair_split in *. inv E. inv H.
-      esplits; eauto.  
-    Qed.
-
-
-    Lemma isim_ctx_aux
-          s i i0 st_src st_tgt st_ctx
-          y fl_src fl_tgt fl_ctx Ist
-          (IN: In (s, i) fl_src /\ In (s, i0) fl_tgt)
-          (SIM: Ist st_src st_tgt
-                ⊢ isim Ist fl_src fl_tgt ibot ibot 
-                    (λ '(st_src, v_src) '(st_tgt, v_tgt), Ist st_src st_tgt ** ⌜v_src = v_tgt⌝) 
-                    false false (st_src, i y) (st_tgt, i0 y))
-      :
-        IstProd Ist IstEq (Any.pair st_src st_ctx) (Any.pair st_tgt st_ctx)
-        ⊢ isim (IstProd Ist IstEq)
-          (addf fl_src fl_ctx) (addf fl_tgt fl_ctx) 
-          ibot ibot
-          (λ '(st_src0, v_src) '(st_tgt0, v_tgt), IstProd Ist IstEq st_src0 st_tgt0 ** ⌜v_src = v_tgt⌝) 
-          false false 
-          (Any.pair st_src st_ctx, translate (emb_ run_l) (i y)) (Any.pair st_tgt st_ctx, translate (emb_ run_l) (i0 y)).
-    Proof.
-      iIntros "H". iDestruct "H" as (? ? ? ?) "(% & IST & %)".
-      des. eapply any_pair_inv in H, H1. des. subst. clear H0.
-      remember (Any.pair st_srcL st_tgtR).
-      remember (Any.pair st_tgtL st_tgtR).
-      iPoseProof (SIM with "IST") as "SIM".
-      Local Transparent isim. iStopProof. uiprop. i.
-      eapply gpaco7_mon; cycle 1.
-      { instantiate (1:= bot7). i. inv PR. }
-      { instantiate (1:= bot7). i. inv PR. }
-      gfinal. right. eapply hpsim_ctx; eauto.
-      ginit. eapply gpaco7_mon; eauto using iunlift_ibot.
-    Qed.
-
-    Theorem isim_ctx
-            ctx ms1 ms2 Ist
-            (SIM: HModSemR.sim ms1 ms2 Ist)
-        :
-            HModSemR.sim (HModSem.add ms1 ctx) (HModSem.add ms2 ctx) (IstProd Ist IstEq).
-    Proof.
-      inv SIM. 
-      econs; ss.
-      { 
-        iIntros "[H C]". iPoseProof (sim_initial with "H") as "[H I]". iFrame.
-        unfold IstProd, IstEq. 
-        iExists (initial_st ms1), (initial_st ms2).
-        iFrame. iPureIntro. esplits; eauto.    
-      }
-      { 
-        unfold add_fnsems. rewrite! List.app_length. rewrite! List.map_length.
-        f_equal. ss.
-      }
-      {
-        i. unfold add_fnsems in MISS. rewrite alist_find_app_o in MISS. des_ifs.
-        admit.
-      }
-      i. unfold add_fnsems in FIND. rewrite alist_find_app_o in FIND. des_ifs.
-      { (* find in ms1 *)
-        admit.
-      }
-      { (* find in ctx *)
-        admit.
-      } 
-    Admitted.
-  End HMODSEM.
-
-  Theorem sim_ctx_hmod
-        ctx md1 md2 Ist
-        (SIM: HModR.sim md1 md2 Ist)
-      :
-        HModR.sim (HMod.add md1 ctx) (HMod.add md2 ctx) (IstProd Ist IstEq).
-  Proof.
-    inv SIM.
-    econs; et.
-    - i. ss. hexploit (sim_modsem sk); et.
-      2: { ii. des. r. eapply isim_ctx. eauto. }
-      unfold Sk.incl, Sk.add in *. i. ss.
-      apply SKINCL.
-      rewrite in_app_iff. et.
-    - r. ss. unfold Sk.add. ss.
-      rewrite sim_sk. et.
+    revert ND k. induction PERM; ss.
+    { i. inv ND. destruct x. rewrite eq_rel_dec_correct. des_ifs. et. }
+    { i. inv ND. inv H3. destruct x, y. rewrite eq_rel_dec_correct. des_ifs.
+      rewrite eq_rel_dec_correct in *. des_ifs. f_equal. exfalso. eapply H2. ss. auto. }
+    { i. rewrite IHPERM1; auto. rewrite IHPERM2; auto.
+      eapply Permutation_NoDup; [|apply ND].
+      eapply Permutation_map. auto.
+    }
   Qed.
-End SIM.
 
-*)
+  Lemma alist_find_comm {K V} `{Dec K}
+        (l0 l1: list (K*V)) fn f
+        (NODUP: NoDup (map fst (l0 ++ l1)))
+        (FIND: alist_find fn (l0 ++ l1) = Some f)
+      :
+        alist_find fn (l1 ++ l0) = Some f.
+  Proof.
+    rewrite alist_find_app_o in *. des_ifs.
+    eapply alist_find_fst_some in Heq, Heq0.
+    rewrite map_app in NODUP.
+    exfalso.
+    eapply NoDup_app_disjoint in NODUP; eauto.
+  Qed.
+
+  Lemma hmod_add_scopes sk md0 md1:
+    HMod.scopes (md0 ★ md1) sk = HMod.scopes md0 sk ++ HMod.scopes md1 sk.
+  Proof. ss. Qed.
+
+  Lemma hmod_add_comm
+    ms0 ms1
+    :
+    HSim.t (ms0 ★ ms1) (ms1 ★ ms0) (const(emp%I))
+      (fun sk => IstSB0 (HMod.scopes (ms0 ★ ms1) sk) perm_Ist).
+  Proof.
+    econs; cycle 1.
+    { rr. eapply Permutation_app_comm. }
+    i. econs; ss.
+    {
+      iIntros "_". iPureIntro. esplits.
+      { eapply (HMod.modsem ms0 ★ ms1 sk).(HModSem.well_scoped_init). }
+      { ii. eapply (HMod.modsem ms0 ★ ms1 sk).(HModSem.well_scoped_init); ss.
+        unfold state_scopes in *. rewrite map_app in *.
+        eapply in_app_or in H. eapply in_or_app. des; eauto.
+      }
+      { eapply Permutation.Permutation_app_comm. }
+    }
+    {
+      r. exists []. rewrite app_nil_l.
+      eapply Permutation.Permutation_app_comm.
+    }
+    { rewrite! app_length. nia. }
+    {
+      i. rewrite map_app in *. eapply in_app_iff, Logic.or_comm.
+      eapply in_app_iff. eauto.
+    }
+
+    ii. eapply alist_find_comm in FIND; cycle 1. 
+    { inv WFT; ss. }
+    esplits; eauto.
+
+    (* simulation *)
+    ii. subst. destruct fs. unfold HModSem.sandbox_body. s.
+    generalize (i y) as it. clear FIND i y.
+    revert NODD. apply combine_quant.
+    revert NODS. apply combine_quant.
+    revert st_tgt. apply combine_quant.
+    revert st_src. apply combine_quant.
+    revert nths. apply combine_quant.
+    eapply isim_coind. i.
+    destruct a as [nths [st_src [st_tgt [NODS [NODD it]]]]]. s.
+    iIntros "(#(_ & CIH) & IST)".
+    assert (CASE := case_itrH _ it); des; subst.
+    - step. iFrame. eauto.
+    - steps_l. steps_r. by_coind "CIH". eauto.
+    - steps_l. force_r. iFrame. by_coind "CIH". eauto.
+    - steps_r. force_l. iFrame. by_coind "CIH". eauto.
+    - destruct s.
+      + step. by_coind "CIH". eauto.
+      + yield "IST"; eauto. by_coind "CIH". eauto.
+      + steps_l. steps_r. by_coind "CIH". eauto.
+    - destruct c. call "IST"; eauto. by_coind "CIH". eauto.
+    - depdes s.
+      + rewrite/__ !HModSB.transl_bind !HModSB.transl_put. des_ifs; cycle 1.
+        { steps_r. force_l. instantiate (1:=q). by_coind "CIH". eauto. }
+        iApply isim_sput_src. iApply isim_sput_tgt.
+        by_coind "CIH". iClear "CIH". unfold perm_Ist. 
+        iDestruct "IST" as "%". des. 
+        iPureIntro. rewrite !state_scopes_update. esplits; eauto. 
+        eapply alist_upd_perm; eauto.
+      + rewrite/__ !HModSB.transl_bind !HModSB.transl_get. des_ifs; cycle 1.
+        { steps_r. force_l. instantiate (1:=q). by_coind "CIH". eauto. }
+        iApply isim_sget_src. iApply isim_sget_tgt.
+        apply existsb_exists in Heq. des. apply String.eqb_eq in Heq0. subst.
+        iAssert (⌜alist_find k st_src = alist_find k st_tgt⌝)%I with "[IST]" as "%".
+        { iDestruct "IST" as "%". des. iPureIntro.
+          eapply alist_permutation_find; eauto. }
+        rewrite H. by_coind "CIH". eauto.
+    - destruct e.
+      + steps_r. force_l. instantiate (1:= q). by_coind "CIH". eauto. 
+      + steps_l. force_r. instantiate (1:= q). by_coind "CIH". eauto. 
+      + step. by_coind "CIH". eauto. 
+    Unshelve. all: eauto. 
+    { eapply alist_upd_nodup. eauto. }
+    { eapply alist_upd_nodup. eauto. }
+  Qed.
+
+  Lemma ctxr_cond_emp_l (m0 m1: HMod.t) P
+    (REF: ctx_refines (m0, (fun _ => emp)%I ∗∗ P) (m1, (fun _ => emp)%I ∗∗ P))
+  :
+    ctx_refines (m0, P) (m1, P).
+  Proof.
+    ii. specialize (REF ctx). destruct ctx. ss.
+    rr in REF. des. rr. esplits; eauto. i.
+    hexploit REF0; eauto; ss.
+    { iIntros "H". iPoseProof (SRC with "H") as "[H0 H1]". iFrame. }
+    i. des.
+    esplits; eauto.
+    iIntros "H". iPoseProof (H0 with "H") as "[[_ H0] H1]". iFrame.
+  Qed.
+  
+  Theorem ctxr_comm (ma mb: HMod.t) P:
+    ctx_refines (HMod.add ma mb, P) (HMod.add mb ma, P).
+  Proof.
+    eapply ctxr_cond_emp_l, ctxr_cond_frameR.
+    eapply main_adequacy. eapply hmod_add_comm.
+  Qed.
+
+End COMM.
