simulations/isim/ISim.v
@@ -18,8 +18,9 @@ Require Import World sWorld.
 From stdpp Require Import coPset gmap.
 
 Require Import HMod SMod.
+Require Import SubPerm.
 
-Require Export ISimCore ITactics.
+Require Export ISimCore ITacticsCore.
 
 Set Implicit Arguments.
 
@@ -129,3 +130,171 @@ Section LEMMAS.
   Qed.
 
 End LEMMAS.
+
+Section HModProd.
+
+  Context `{Σ: GRA.t}.
+
+  Definition IstProd0 (IstL IstR : nat -> alist key Any.t -> alist key Any.t -> iProp) :=
+    fun nths (st_src st_tgt: alist key Any.t) =>
+      (∃ st_srcL st_tgtL st_srcR st_tgtR,
+       ⌜st_src = st_srcL ++ st_srcR /\ st_tgt = st_tgtL ++ st_tgtR⌝ ∗
+       IstL nths st_srcL st_tgtL ∗ IstR nths st_srcR st_tgtR)%I.
+
+  Definition IstProd IstL IstR :=
+    fun (sk: Sk.t) => IstProd0 (IstL sk) (IstR sk).
+
+  Definition IstSB0 scopes (Ist: nat -> alist key Any.t -> alist key Any.t -> iProp) :=
+    fun nths st_src st_tgt =>
+      (⌜incl (state_scopes st_src) scopes ∧
+        incl (state_scopes st_tgt) scopes⌝
+       ∗ Ist nths st_src st_tgt)%I.
+
+  Definition IstSB ms Ist :=
+    fun (sk: Sk.t) => IstSB0 (HMod.scopes ms sk) (Ist sk).
+
+  Definition IstEq0 : nat -> alist key Any.t -> alist key Any.t -> iProp :=
+    (fun _ st_src st_tgt => ⌜st_src = st_tgt⌝)%I.
+
+  Definition IstEq :=
+    fun (sk: Sk.t) => IstEq0.
+
+  Lemma state_scopes_update k v st:
+    state_scopes (alist_upd k v st) = state_scopes st.
+  Proof.
+    rewrite /state_scopes -!List.map_map alist_upd_keys. eauto.
+  Qed.
+  
+  Lemma isim_reflR Ist fl_src fl_tgt scopesL scopesR scopesF (EqR: _->_->_->iProp) itr
+    (DISJ: List.NoDup (scopesL ++ scopesR))
+    (INCL: incl scopesF scopesR)
+    (EQGET: ∀ nths st_src st_tgt,
+        EqR nths st_src st_tgt -∗ ⌜st_src = st_tgt⌝)
+    (EQSET: ∀ nths st_src st_tgt nths0 (k: key) v,
+        EqR nths st_src st_tgt -∗
+          EqR nths0 (alist_upd k v st_src) (alist_upd k v st_tgt))
+    :
+    isim_fsem fl_src fl_tgt (IstProd0 (IstSB0 scopesL Ist) EqR)
+      (HModSem.sandbox_body (scopesF,itr)) (HModSem.sandbox_body (scopesF,itr)).
+  Proof.
+    ii. subst. unfold HModSem.sandbox_body. s.
+    generalize (itr y) as it; clear itr y.
+    revert NODD. apply combine_quant.
+    revert NODS. apply combine_quant.
+    revert st_tgt. apply combine_quant.
+    revert st_src. apply combine_quant.
+    revert nths. apply combine_quant.
+    eapply isim_coind. i. destruct a as [nths [st_src [st_tgt [NODS [NODD it]]]]]. s.
+    iIntros "(#(_ & CIH) & IST)".
+    assert (CASE := case_itrH _ it); des; subst.
+    - step. iFrame. eauto.
+    - steps_l. steps_r. by_coind "CIH". eauto.
+    - steps_l. force_r. iFrame. by_coind "CIH". eauto.
+    - steps_r. force_l. iFrame. by_coind "CIH". eauto.
+    - depdes s.
+      + step. by_coind "CIH". iApply IMON; [|eauto]; nia.
+      + yield "IST"; eauto. by_coind "CIH". eauto.
+      + steps_l. steps_r. by_coind "CIH". eauto.
+    - destruct c. call "IST"; eauto. by_coind "CIH". eauto.
+    - depdes s.
+      + rewrite/__ !HModSB.transl_bind !HModSB.transl_put. des_ifs; cycle 1.
+        { steps_r. force_l. instantiate (1:=q). by_coind "CIH". eauto. }
+        iApply isim_sput_src. iApply isim_sput_tgt.
+        by_coind "CIH". iClear "CIH". unfold IstProd.
+        iDestruct "IST" as (? ? ? ?) "(% & (% & IST) & EQR)". des; subst.
+        apply existsb_exists in Heq. des. apply String.eqb_eq in Heq0. subst.
+        iExists st_srcL, st_tgtL, (alist_upd k v st_srcR), (alist_upd k v st_tgtR).
+        iSplitR; cycle 1.
+        { iFrame. iSplit; eauto. iApply EQSET. eauto. }
+        iPureIntro. esplits; eauto.
+        * eapply alist_upd_tail. ii. 
+          eapply NoDup_app_disjoint; try apply DISJ; eauto.
+          eapply H0. eapply in_map in H. rewrite map_map in H. apply H.
+        * eapply alist_upd_tail. ii.
+          eapply NoDup_app_disjoint; try apply DISJ; eauto.
+          apply H1. eapply in_map in H. rewrite map_map in H. apply H.
+      + rewrite/__ !HModSB.transl_bind !HModSB.transl_get. des_ifs; cycle 1.
+        { steps_r. force_l. instantiate (1:=q). by_coind "CIH". eauto. }
+        iApply isim_sget_src. iApply isim_sget_tgt.
+        apply existsb_exists in Heq. des. apply String.eqb_eq in Heq0. subst.
+        iAssert (⌜alist_find k st_src = alist_find k st_tgt⌝ ∗
+                 IstProd0 (IstSB0 scopesL Ist) EqR nths st_src st_tgt)%I
+          with "[IST]" as "(% & IST)".
+        { iDestruct "IST" as (? ? ? ?) "(% & (% & IST) & EQR)". des; subst.
+          iPoseProof (EQGET with "EQR") as "%". subst.
+          iSplitR; cycle 1.
+          { repeat iExists _. iFrame. eauto. }
+          rewrite alist_find_app_o; des_ifs.
+          { exfalso. apply alist_find_fst_some in Heq0.
+            eapply NoDup_app_disjoint; try apply DISJ; eauto.
+            apply H0. eapply in_map in Heq0. rewrite map_map in Heq0. eauto.
+          }
+          rewrite alist_find_app_o; des_ifs.
+          exfalso. apply alist_find_fst_some in Heq1.
+          eapply NoDup_app_disjoint; try apply DISJ; eauto.
+          apply H1. eapply in_map in Heq1. rewrite map_map in Heq1. eauto.
+        }
+        rewrite H. by_coind "CIH". eauto.
+    - destruct e.
+      + steps_r. force_l. instantiate (1:=q). by_coind "CIH". eauto.
+      + steps_l. force_r. instantiate (1:=q). by_coind "CIH". eauto.
+      + step. by_coind "CIH". eauto.
+  Unshelve. all: eauto.
+  { eapply alist_upd_nodup. eauto. }
+  { eapply alist_upd_nodup. eauto. }
+  Qed.
+
+  Lemma mod_sim_reflR A B C init_cond Ist
+    (INIT: ∀ sk, init_cond sk -∗
+                    IstProd (IstSB A Ist) IstEq sk 1
+                    (HModSem.initial_st (HMod.modsem (HMod.add A C) sk))
+                    (HModSem.initial_st (HMod.modsem (HMod.add B C) sk)))
+    (MON: ∀ sk nths nths' (LE: nths <= nths') st_src st_tgt,
+        Ist sk nths st_src st_tgt -∗ Ist sk nths' st_src st_tgt)
+    (SCOPE: ∀ sk, sub_perm (HMod.scopes B sk) (HMod.scopes A sk))
+    (LEN: ∀ sk, List.length (HModSem.fnsems (HMod.modsem A sk)) =
+                List.length (HModSem.fnsems (HMod.modsem B sk)))
+    (MATCH: ∀ sk fn,
+           In fn (List.map fst (HModSem.fnsems (HMod.modsem A sk))) →
+           In fn (List.map fst (HModSem.fnsems (HMod.modsem B sk))))
+    (SIM: ∀ sk fn
+            (IN: In fn (List.map fst (HModSem.fnsems (HMod.modsem A sk)))),
+          HSSim.sim_fun (HMod.modsem (HMod.add A C) sk) (HMod.modsem (HMod.add B C) sk)
+            (IstProd (IstSB A Ist) IstEq sk) fn)
+    (SK: HMod.sk A = HMod.sk B)
+    :
+    HSim.t (HMod.add A C) (HMod.add B C) init_cond (IstProd (IstSB A Ist) IstEq).
+  Proof.
+    econs; cycle 1.
+    { rr. eapply Permutation_app_tail. rewrite SK. refl. }
+    econs.
+    - apply INIT.
+    - i. iIntros "H". iDestruct "H" as (? ? ? ?) "(% & (% & H) & %)"; des; subst.
+      do 4 (iExists _). do 2 (iSplit; eauto). iSplitR; eauto.
+      iApply MON; [|eauto]; nia.
+    - s. apply sub_perm_cancel_tail. eapply SCOPE.
+    - s. rewrite !app_length. rewrite LEN. eauto.
+    - s. i. rewrite map_app in *. apply in_or_app. apply in_app_or in IN.
+      des; eauto.
+    - s. i. rewrite map_app in IN. apply in_app_or in IN. des.
+      { eapply SIM; eauto. }
+      ii. exists fs. destruct fs as [scp f].
+      assert (FND: alist_find fn (HModSem.fnsems (HMod.modsem C sk))
+                   = Some (scp,f)).
+      { s in FIND. rewrite alist_find_app_o in FIND. des_ifs.
+        exfalso. assert (ND:= HModSem.wf_fns WFS). s in ND. rewrite map_app in ND.
+        eapply NoDup_app_disjoint; try apply ND; eauto.
+        eapply alist_find_some, (in_map fst) in Heq. eauto.
+      }
+
+      split.
+      { eapply alist_find_some_iff; eauto.
+        apply in_or_app. right. eapply alist_find_some. eauto. }
+      
+      eapply isim_reflR; eauto.
+      + apply WFS.
+      + ii. eapply (HMod.modsem C sk). unfold fnsems_scopes. rewrite FND. eauto.
+      + i. unfold IstEq, IstEq0. iIntros "%". subst. eauto.
+Qed.
+  
+End HModProd.
