simulations/isim/ISimFacts.v
@@ -1,0 +1,110 @@
+Require Import Coqlib sflib ITreelib.
+Require Import AList SubPerm.
+Require Import PCM IPM.
+Require Import Mod HMod.
+
+From ExtLib Require Import
+     Data.Map.FMapAList.
+
+Require Import ModSim HPSimFacts ISimCore.
+
+
+Section HSSIM_ADEQUACY.
+
+  Context `{Σ: GRA.t}.
+
+  Lemma hssim_wf ms mt cond Ist
+    (SIM: HSSim.t ms mt cond Ist)
+    (WF: HModSem.wf ms)
+    :
+    HModSem.wf mt.
+  Proof.
+    inv SIM. econs.
+    - eapply in_eqlen_nodup_rev with (l1:= map fst _).
+      + rewrite map_length. rewrite sim_length. rewrite map_length. eauto.
+      + apply WF.
+      + eauto.
+    - eapply sub_perm_nodup; eauto. apply WF.
+  Qed.
+
+  Lemma hssim_match ms mt cond Ist fn
+    (SIM: HSSim.t ms mt cond Ist)
+    (WF: List.NoDup (List.map fst (HModSem.fnsems ms)))
+    (IN: In fn (List.map fst (HModSem.fnsems mt)))
+    :
+    In fn (List.map fst (HModSem.fnsems ms)).
+  Proof.
+    eapply nodup_eqlen_in_rev, IN.
+    - rewrite !map_length. eapply SIM.
+    - eauto.
+    - i. eapply SIM. eauto.
+  Qed.
+  
+  Lemma hssim_adequacy
+    (ms mt: HModSem.t) (p q: Σ)
+    (IC: iProp) Ist
+
+    (WF: URA.wf (p ⋅ q))
+    (COND: IC p)
+    (WFS: HModSem.wf ms)
+    (WFT: HModSem.wf mt)
+    (SIM: HSSim.t ms mt IC Ist)
+    :
+    MSim.t (HModSem.to_mod ms (p ⋅ q)) (HModSem.to_mod mt q).
+  Proof.
+    inv SIM.
+    econs; i; ss.
+    - ii; subst; eauto.
+    - instantiate (1:= interp_inv Ist).
+      inv WF0. econs; eauto.
+      iIntros "H". iMod (MR with "H") as "H". iModIntro.
+      iStopProof. eauto.
+    - instantiate (1:= ε).
+      inv WF0. econs; eauto.
+      iIntros "H". iMod (MRS with "H") as "H". iModIntro.
+      unfold ctx_sem. rewrite foldr_app. s. r_solve. eauto.
+    - eexists ε. econs; eauto.
+      { instantiate (1:= p). s. r_solve. eauto. }
+      {
+        iIntros "H". iModIntro.
+        eapply iProp_Own in COND. iApply sim_initial.
+        iApply COND. eauto.
+      }
+      { eapply ms.(HModSem.nodup_fns). eapply WFS. }
+      { eapply mt.(HModSem.nodup_fns). eapply WFT. }
+    - rewrite! map_length. eauto.
+    - rewrite alist_find_map_snd in *. unfold o_map in *. des_ifs; cycle 1.
+      { exfalso.
+        eapply alist_find_fst_some, sim_match, alist_find_fst_in in Heq0.
+        des. rewrite Heq in Heq0. ss.
+      }
+      esplits; eauto.
+      exploit sim_fnsems; eauto using alist_find_fst_some.
+      { apply WFS. }
+      { apply WFT. }
+
+      ii. des; subst.
+      rewrite Heq in x0. inv x0. inv SIMMRS.
+      eapply hpsim_adequacy; eauto; cycle 5.
+      { ginit. i.
+        eapply gpaco8_mon with (r:= iunlift ibot) (rg:= iunlift ibot); eauto using iunlift_ibot.
+        eapply isim_init; eauto.
+        iIntros "H". iApply isim_upd. iPoseProof (MR with "H") as ">H".
+        iModIntro. iApply x1; eauto.
+      }
+      { r_solve; eauto. }
+      { r_solve; eauto. }
+      { inv WFS. rewrite List.map_map.
+        eapply eq_ind; [apply wf_fns|].
+        f_equal. extensionalities. destruct H; eauto.
+      }
+      { inv WFT. rewrite List.map_map.
+        eapply eq_ind; [apply wf_fns|].
+        f_equal. extensionalities. destruct H; eauto.
+      }
+      { rewrite List.map_map. f_equal. extensionalities. destruct H. eauto. }
+      { rewrite List.map_map. f_equal. extensionalities. destruct H. eauto. }
+      { apply le_mine_refl. ii; eauto. }
+  Qed.
+  
+End HSSIM_ADEQUACY.
