simulations/isim/ITacticsCore.v
@@ -1,0 +1,645 @@
+Require Import Coqlib ITreelib sflib.
+Require Import Events STS.
+Require Import Behavior.
+
+Require Import Skeleton.
+Require Import PCM IPM STB.
+Require Import Any.
+
+Require Import Relation_Definitions.
+Require Import Relation_Operators.
+Require Import RelationPairs.
+From ExtLib Require Import
+     Data.Map.FMapAList.
+Require Import Red IRed.
+Require Import HPSim.
+Require Import World sWorld.
+Require Import ISimCore.
+Require Import Events Mod SMod HMod PMod.
+Require Import SubPerm.
+Require Import LAuto.
+
+From stdpp Require Import coPset gmap.
+
+(************ User Tactics **************)
+
+Lemma string_app_inv
+  p s s'
+  (EQ: (p ++ s = p ++ s')%string)
+  :
+  (s = s')%string.
+Proof.
+  revert_until p. induction p; i; ss.
+  unfold append in EQ. depdes EQ. eauto.
+Qed.
+
+Ltac inv_string X :=
+  inv X;
+  repeat match goal with [H: @eq string _ _|-_] =>
+           apply string_app_inv in H
+    end; ss.
+
+Ltac prove_scope :=
+  try unfold HModSem.fnsems; try unfold SModSem.fnsems; try unfold fnsems_scopes;
+  s; ii; des_ifs; ss; des; ss; eauto.
+
+Ltac prove_nodup :=
+  repeat (econs; [ii; ss; des; try match goal with [H: _ |- _] => inv_string H end|]); try (econs; fail).
+
+Ltac by_coind CIH :=
+  iApply isim_progress; iApply isim_base;
+  iSpecialize (CIH $! _); repeat instantiate (1:= existT _ _); s;
+  iApply CIH.
+
+Ltac unfold_hmod :=
+  match goal with
+  | [|-context[HMod.modsem ?x _]] => rewrite/__ {1}/x; progress unseal "ccr"
+  | [|-context[HMod.sk ?x]] => rewrite/__ {1}/x; progress unseal "ccr" end.
+
+Lemma ereplace T (x y: T):
+  x = y -> x = y.
+Proof. eauto. Qed.
+
+Ltac alist_upd_simpl nodup_tac :=
+  match goal with
+  [ |- context[alist_upd ?k ?v ?l]] =>
+    match l with
+    | context[(k,?v0)] =>
+      let TMP := fresh "_TMP" in
+      let NODUP := fresh "NODUP" in
+      match goal with [H: List.NoDup _|-_] =>
+        eassert (TMP: List.NoDup (List.map fst l)) by (nodup_tac H); clear H; revert TMP
+      end;
+      erewrite (@ereplace _ l); [intros ?|Lauto_prepare; Lauto_find (k,v0); refl];
+      eassert (NODUP := alist_upd_nodup k v _ TMP); revert NODUP;
+      rewrite !alist_upd_with_nodup; [|exact TMP]; clear TMP;
+      Lauto_finish; intros ?
+    end
+  end.
+
+Ltac trivial_nodup H :=
+  exact H.
+
+Ltac alist_find_simpl nodup_tac :=
+  match goal with
+  [ |- context[alist_find ?k ?l]] =>
+    match l with
+    | context[(k,_)] =>
+      let TMP := fresh "_TMP" in
+      match goal with [H: List.NoDup _|-_] =>
+        eassert (TMP: List.NoDup (List.map fst l))  by (nodup_tac H);
+        revert TMP
+      end;
+      erewrite (@ereplace _ l);
+      [intros ?
+      |Lauto_normalize; try rewrite !List.map_app; simpl List.map; Lauto_prepare;
+       match goal with [|-context[(k,?v)]] => Lauto_find (k,v) end; refl];
+      rewrite !alist_find_with_nodup; [|exact TMP]; clear TMP;
+      Lauto_finish
+    end
+  end.
+  
+Lemma map_map_compose {A B C} (f: A -> B) (g: B -> C) l:
+  List.map g (List.map f l) = List.map (g ∘ f) l.
+Proof.
+  rewrite List.map_map. refl.
+Qed.
+
+Lemma fst_map_snd {A B C} f:
+  (fst ∘ @map_snd A B C f) = fst.
+Proof.
+  extensionalities. destruct H. s. eauto.
+Qed.
+
+Ltac fnsems_nodup H :=
+  revert H; simpl HModSem.fnsems; repeat unfold_hmod; simpl List.map;
+  try rewrite !map_map_compose; try rewrite !fst_map_snd; eauto; fail.
+
+Ltac hss :=
+  ss;
+  try (rewrite !Any.pair_split in * );
+  try (rewrite !Any.upcast_downcast in * );
+  repeat (match goal with [G: Any.downcast _ = Some _ |-_] =>
+    apply Any.downcast_upcast in G; inv G; ss
+   end);
+  repeat (match goal with [G: Any.upcast (_:?T) = Any.upcast (_:?T) |-_] =>
+    apply Any.upcast_inj in G; destruct G as [_ G]; red in G; depdes G; ss
+   end);
+  repeat (match goal with [G: Some _ = Some _ |- _] =>
+    depdes G; ss
+  end);
+  try (rewrite !Any.pair_split in * );
+  try (rewrite !Any.upcast_downcast in * );
+  repeat (alist_upd_simpl trivial_nodup); s.
+
+(***
+  Step-level tactics
+ ***)
+
+Ltac iIntrosFresh H := iIntros H || iIntrosFresh (H ++ "'")%string.
+
+Ltac des_pairs :=
+  repeat match goal with
+    | [H: context[let (_, _) := ?x in _] |- _] =>
+        let n0 := fresh x in let n1 := fresh x in destruct x as [n0 n1]
+    | |- context[let (_, _) := ?x in _] =>
+        let n0 := fresh x in let n1 := fresh x in destruct x as [n0 n1]
+    end.
+
+Ltac desugar itr :=
+  match itr with
+  | HoareBody _ _ _ => rewrite/__ {1}/itr
+  | HoareCall _ _ _ _ _ => rewrite/__ {1}/itr
+  | HoareSpawn _ _ _ => rewrite/__ {1}/itr
+  | HoareYield _ _ => rewrite/__ {1}/itr
+  | cput _ _ => rewrite/__{1}/itr
+  | cgetU _ => rewrite/__{1}/itr
+  | cgetN _ => rewrite/__{1}/itr
+  | triggerUB => rewrite/__{1}/itr
+  | triggerNB => rewrite/__{1}/itr
+  end.
+
+Ltac _unwrapSB itr :=
+  match itr with
+  | Ret _ =>
+      rewrite HModSB.transl_ret
+  | tau;; _ =>
+      rewrite HModSB.transl_tau
+  | trigger (Choose _) => 
+      rewrite HModSB.transl_core
+  | trigger (Take _) => 
+      rewrite HModSB.transl_core
+  | trigger (IO _ _) => 
+      rewrite HModSB.transl_core  
+  | trigger (Call _ _) =>
+      rewrite HModSB.transl_call
+  | trigger (SPut _ _) =>
+      idtac
+  | trigger (SGet _) =>
+      idtac
+  | trigger (Assume _) => 
+      rewrite HModSB.transl_ag
+  | trigger (Guarantee _) => 
+      rewrite HModSB.transl_ag
+  | unwrapU _ =>
+      rewrite HModSB.transl_unwrapU
+  | unwrapN _ =>
+      rewrite HModSB.transl_unwrapN
+  | assume _ =>
+      rewrite HModSB.transl_asm
+  | guarantee _ =>
+      rewrite HModSB.transl_guar
+  | trigger (Spawn _ _) =>
+      rewrite HModSB.transl_sch
+  | trigger (Yield _) =>
+      rewrite HModSB.transl_sch
+  | trigger Tid =>
+      rewrite HModSB.transl_sch
+  | HoareAPC _ _ =>
+      idtac
+  | _ => fail
+  end.
+
+Ltac unwrapSB :=
+  try match goal with
+  | [|-context[HModSem.sandbox _ ?itr]] => first [desugar itr|fail 2]
+  end;
+  match goal with
+  | [|-context[HModSem.sandbox _ (?itr >>= _)]] =>
+      rewrite HModSB.transl_bind; unwrapSB
+  | [|-context[HModSem.sandbox _ ?itr]] => first [_unwrapSB itr|fail 2]
+  end.
+
+Ltac _unwrapS itr :=
+  match itr with
+  | Ret _ =>
+      rewrite SModRed.interp_ret
+  | tau;; _ =>
+      rewrite SModRed.interp_tau
+  | trigger (Choose _) => 
+      rewrite SModRed.interp_core
+  | trigger (Take _) => 
+      rewrite SModRed.interp_core
+  | trigger (IO _ _) => 
+      rewrite SModRed.interp_core  
+  | trigger (Call _ _) =>
+      rewrite/__ SModRed.interp_call {1}/handle_callE_hmodE
+  | trigger (Spawn _ _) =>
+      rewrite/__ SModRed.interp_sch {1}/handle_schE_hmodE
+  | trigger (Yield _) =>
+      rewrite/__ SModRed.interp_sch {1}/handle_schE_hmodE
+  | trigger Tid =>
+      rewrite/__ SModRed.interp_sch {1}/handle_schE_hmodE
+  | trigger (SPut _ _) =>
+      rewrite SModRed.interp_pg
+  | trigger (SGet _) =>
+      rewrite SModRed.interp_pg
+  | trigger (Assume _) => 
+      rewrite SModRed.interp_ag
+  | trigger (Guarantee _) => 
+      rewrite SModRed.interp_ag
+  | unwrapU _ =>
+      rewrite SModRed.interp_unwrapU
+  | unwrapN _ =>
+      rewrite SModRed.interp_unwrapN
+  | assume _ =>
+      rewrite SModRed.interp_asm
+  | guarantee _ =>
+      rewrite SModRed.interp_guar
+  | trigger APC =>
+      (* idtac *)
+      rewrite/__ SModRed.interp_apc {1}/handle_apcE_hmodE
+  | _ => fail
+  end.
+
+Ltac unwrapS :=
+  try match goal with
+    | [|-context[interp_smod _ _ _ ?itr]] => first [desugar itr|fail 2]
+  end;
+  match goal with
+  | [|-context[interp_smod _ _ _ (?itr >>= _)]] =>
+      rewrite SModRed.interp_bind; unwrapS
+  | [|-context[interp_smod _ _ _ ?itr]] => first [_unwrapS itr|fail 2]
+  end.
+
+Ltac _unwrapP itr :=
+  match itr with
+  | Ret _ =>
+      rewrite PModRed.transl_ret
+  | tau;; _ =>
+      rewrite PModRed.transl_tau
+  | trigger (Choose _) => 
+      rewrite PModRed.transl_core
+  | trigger (Take _) => 
+      rewrite PModRed.transl_core
+  | trigger (IO _ _) => 
+      rewrite PModRed.transl_core  
+  | trigger (Call _ _) =>
+      rewrite PModRed.transl_call
+  | trigger (Spawn _ _) =>
+      rewrite PModRed.transl_sch
+  | trigger (Yield _) =>
+      rewrite PModRed.transl_sch
+  | trigger Tid =>
+      rewrite PModRed.transl_sch
+  | trigger (SPut _ _) =>
+      rewrite PModRed.transl_pg
+  | trigger (SGet _) =>
+      rewrite PModRed.transl_pg
+  | unwrapU _ =>
+      rewrite PModRed.transl_unwrapU
+  | unwrapN _ =>
+      rewrite PModRed.transl_unwrapN
+  | assume _ =>
+      rewrite PModRed.transl_asm
+  | guarantee _ =>
+      rewrite PModRed.transl_guar
+  | _ => fail
+  end.
+
+Ltac unwrapP :=
+  try match goal with
+  | [|-context[PModSem.transl ?itr]] => first [desugar itr|fail 2]
+  end;
+  match goal with
+  | [|-context[PModSem.transl (?itr >>= _)]] =>
+      rewrite PModRed.transl_bind; unwrapP
+  | [|-context[PModSem.transl ?itr]] => first [_unwrapP itr|fail 2]
+  end.
+
+Ltac unfold_precond_postcond term := let TM := fresh "_term" in
+  set (TM := term) at 1;
+  repeat (unfold precond in TM; simpl in TM);
+  repeat (unfold postcond in TM; simpl in TM);
+  subst TM.
+
+Ltac _step_l :=
+  match goal with
+  (******* isim ******)
+  (** src **)
+  | [ |- environments.envs_entails _ (isim _ _ _ _ _ _ _ _ _ _ (_, tau;; _) _) ] =>
+      iApply isim_tau_src
+  | [ |- environments.envs_entails _ (isim _ _ _ _ _ _ _ _ _ _ (_, Ret _ >>= _) _) ] =>
+      rewrite bind_ret_l
+  | [ |- environments.envs_entails _ (isim _ _ _ _ _ _ _ _ _ _ (_, (HModSem.sandbox _ (trigger (SPut _ _))) >>= _) _) ] =>
+      iApply isim_sput_src_sandbox; [s;eauto|]
+  | [ |- environments.envs_entails _ (isim _ _ _ _ _ _ _ _ _ _ (_, (HModSem.sandbox _ (trigger (SGet _))) >>= _) _) ] =>
+      iApply isim_sget_src_sandbox; [s;eauto|]
+  | [ |- environments.envs_entails _ (isim _ _ _ _ _ _ _ _ _ _ (_, trigger (Take _) >>= _) _) ] =>
+      let name := fresh "q" in
+      iApply isim_take_src; iIntros (name)
+  | [ |- environments.envs_entails _ (isim _ _ _ _ _ _ _ _ _ _  (_, trigger (Assume ?P) >>= _) _) ] =>
+      unfold_precond_postcond P; iApply isim_Assume_src; iIntrosFresh "ASM"
+  | [ |- environments.envs_entails _ (isim _ _ _ _ _ _ _ _ _ _ (_, unwrapU ?ox >>= _) _) ] =>
+      let name := fresh "q" in
+      iApply isim_unwrapU_src; iIntros (name) "%";
+      match goal with [ H: ?x = Some _ |- _ ] => let G := fresh "G" in rename H into G; try rewrite G in * end
+  | [ |- environments.envs_entails _ (isim _ _ _ _ _ _ _ _ _ _ (_, assume _ >>= _) _) ] =>
+      let name := fresh "asm" in iApply isim_asm_src; iIntros (name)
+  | [ |- environments.envs_entails _ (isim _ _ _ _ _ _ _ _ _ _ (_, trigger Tid >>= _) _) ] =>
+      iApply isim_tid_src
+  | [ |- environments.envs_entails _ (isim _ _ _ _ _ _ _ _ _ _ (_, HModSem.sandbox _ (HoareAPC _ _) >>= _) _) ] =>
+      idtac
+  end.
+
+Ltac _step_r :=
+  match goal with
+  (******* isim ******)
+  (** tgt **)
+  | [ |- environments.envs_entails _ (isim _ _ _ _ _ _ _ _ _ _ _ (_, Ret _ >>= _)) ] =>
+      rewrite bind_ret_l
+  | [ |- environments.envs_entails _ (isim _ _ _ _ _ _ _ _ _ _ _ (_, tau;; _)) ] =>
+      iApply isim_tau_tgt
+  | [ |- environments.envs_entails _ (isim _ _ _ _ _ _ _ _ _ _ _ (_, (HModSem.sandbox _ (trigger (SPut _ _))) >>= _)) ] =>
+      iApply isim_sput_tgt_sandbox; [s; eauto|]
+  | [ |- environments.envs_entails _ (isim _ _ _ _ _ _ _ _ _ _ _ (_, (HModSem.sandbox _ (trigger (SGet _))) >>= _)) ] =>
+      iApply isim_sget_tgt_sandbox; [s; eauto|]
+  | [ |- environments.envs_entails _ (isim _ _ _ _ _ _ _ _ _ _ _ (_, trigger (Choose _) >>= _)) ] =>
+      let name := fresh "q" in
+      iApply isim_choose_tgt; iIntros (name)
+  | [ |- environments.envs_entails _ (isim _ _ _ _ _ _ _ _ _ _ _ (_, trigger (Guarantee ?P) >>= _)) ] =>
+      unfold_precond_postcond P; iApply isim_Guarantee_tgt; iIntrosFresh "GRT"
+  | [ |- environments.envs_entails _ (isim _ _ _ _ _ _ _ _ _ _ _ (_, unwrapN ?ox >>= _)) ] =>
+      let name := fresh "q" in
+      iApply isim_unwrapN_tgt; iIntros (name) "%";
+      match goal with [ H: ?x = Some _ |- _ ] => let G := fresh "G" in rename H into G; try rewrite G in * end
+  | [ |- environments.envs_entails _ (isim _ _ _ _ _ _ _ _ _ _ _ (_, guarantee _ >>= _)) ] =>
+      let name := fresh "grt" in iApply isim_guar_tgt; iIntros (name)
+  | [ |- environments.envs_entails _ (isim _ _ _ _ _ _ _ _ _ _ _ (_, trigger Tid >>=  _)) ] =>
+      iApply isim_tid_tgt
+  | [ |- environments.envs_entails _ (isim _ _ _ _ _ _ _ _ _ _ _ (_, HModSem.sandbox _ (HoareAPC _ _) >>= _)) ] =>
+      idtac
+  end.
+
+Ltac _step :=
+  match goal with
+  (******* isim ******)
+  (** both **)
+  | [ |- environments.envs_entails _ (isim _ _ _ _ _ _ _ _ _ _ (_, Ret _) (_, Ret _)) ] =>
+      iApply isim_ret
+  | [ |- environments.envs_entails _ (isim _ _ _ _ _ _ _ _ _ _ (_, trigger (IO _ _) >>= _) (_, trigger (IO _ _) >>= _)) ] =>
+      iApply isim_io; iIntros "%"
+  | [ |- environments.envs_entails _ (isim _ _ _ _ _ _ _ _ _ _ (_, trigger (Spawn _ _) >>= _) (_, trigger (Spawn _ _) >>= _)) ] =>
+      iApply isim_spawn
+  end.
+
+Ltac _force_l :=
+  match goal with
+  | [ |- environments.envs_entails _ (isim _ _ _ _ _ _ _ _ _ _ (_, trigger (Choose ?T) >>= _) _) ] =>
+      iApply isim_choose_src
+  | [ |- environments.envs_entails _ (isim _ _ _ _ _ _ _ _ _ _ (_, trigger (Guarantee ?P) >>= _) _) ] =>
+      unfold_precond_postcond P; iApply isim_Guarantee_src
+  | [ |- environments.envs_entails _ (isim _ _ _ _ _ _ _ _ _ _ (_, unwrapN _ >>= _) _) ] =>
+      iApply isim_unwrapN_src; iExists _
+  | [ |- environments.envs_entails _ (isim _ _ _ _ _ _ _ _ _ _ (_, guarantee _ >>= _) _) ] =>
+      iApply isim_guar_src
+  end
+.
+
+Ltac _force_r :=
+  match goal with
+  | [ |- environments.envs_entails _ (isim _ _ _ _ _ _ _ _ _ _ _ (_, trigger (Take _) >>= _)) ] =>
+      iApply isim_take_tgt
+  | [ |- environments.envs_entails _ (isim _ _ _ _ _ _ _ _ _ _ _ (_, trigger (Assume ?P) >>= _)) ] =>
+      unfold_precond_postcond P; iApply isim_Assume_tgt
+  | [ |- environments.envs_entails _ (isim _ _ _ _ _ _ _ _ _ _ _ (_, unwrapU _ >>= _)) ] =>
+      iApply isim_unwrapU_tgt; iExists _
+  | [ |- environments.envs_entails _ (isim _ _ _ _ _ _ _ _ _ _ _ (_, assume _ >>= _)) ] =>
+      iApply isim_asm_tgt
+  end
+.
+
+
+Ltac hide_itree_l := let IT := fresh "ITREE" in
+  match goal with [|- _ (_ ?it _)] => set (IT := it) end; try unfold IT at 2.
+Ltac hide_itree_r := let IT := fresh "ITREE" in
+  match goal with [|- _ (_ _ ?it)] => set (IT := it) end; first [ try (unfold IT at 2; fail 1) | unfold IT at 1].
+Ltac show_itree :=
+  match goal with [IT:=_ |-_] => unfold IT; clear IT end.
+
+Ltac unfold_stb :=
+  try match goal with
+    [|-context[unwrapN (?stb ?sk ?name)]] =>
+      try match goal with
+        [H: context[stb_incl _ (stb _)]|-_] =>
+          let RW := fresh "_RW" in let ND := fresh "_ND" in
+          edestruct H as [ND RW];
+          erewrite (RW name);
+          [|revert ND; unfold to_stb;
+            match goal with [|-context[alist_find _ ?x]] => rewrite/__ /x end;
+            unseal "ccr"; i;
+            alist_find_simpl fnsems_nodup;
+            refl];
+          simpl unwrapN; clear ND RW
+      end
+  end.
+
+Ltac prep :=
+  first
+    [ unwrapSB
+    | unwrapS; unfold_stb; unwrapSB
+    | unwrapP; unwrapSB
+    | idtac];
+  try rewrite !bind_bind;
+  try rewrite !bind_tau.
+
+Ltac step_l :=
+  hide_itree_r;
+  prep; _step_l; try alist_find_simpl fnsems_nodup; des_pairs; s;
+  show_itree.
+
+Ltac step_r :=
+  hide_itree_l;
+  prep; _step_r; try alist_find_simpl fnsems_nodup; des_pairs; s;
+  show_itree.
+
+Ltac step :=
+  hide_itree_r; prep; show_itree;
+  hide_itree_l; prep; show_itree;
+  _step; des_pairs; s.
+
+Ltac force_l :=
+  hide_itree_r;
+  prep; _force_l; s;
+  show_itree.
+  
+Ltac force_r :=
+  hide_itree_l;
+  prep; _force_r; s;
+  show_itree.
+  
+Ltac steps_l :=
+  repeat step_l.
+  (* hide_itree_r; *)
+  (* repeat (prep; _step_l; try alist_find_simpl fnsems_nodup; des_pairs; s); *)
+  (* show_itree. *)
+Ltac steps_r :=
+  repeat step_r.
+  (* hide_itree_l; *)
+  (* repeat (prep; _step_r; try alist_find_simpl fnsems_nodup; des_pairs; s); *)
+  (* show_itree. *)
+
+Ltac inline_l :=
+  hide_itree_r;
+  prep;
+  iApply isim_inline_src;
+  [simpl HModSem.fnsems; repeat unfold_hmod; simpl List.map;
+   alist_find_simpl fnsems_nodup; eauto|];
+  unfold interp_sb_hp, HoareFun; s;
+  show_itree.
+  
+Ltac inline_r :=
+  hide_itree_l;
+  prep;
+  iApply isim_inline_tgt;
+  [simpl HModSem.fnsems; repeat unfold_hmod; simpl List.map;
+   alist_find_simpl fnsems_nodup; eauto|];
+  unfold interp_sb_hp, HoareFun; s;
+  show_itree.
+
+Ltac call hyps :=
+  hide_itree_r; prep; show_itree;
+  hide_itree_l; prep; show_itree;
+  iApply isim_call;
+  iSplitL hyps; [ |iIntros "% % % % % %"; iIntrosFresh "IST"].
+
+Ltac yield hyps :=
+  hide_itree_r; prep; show_itree;
+  hide_itree_l; prep; show_itree;
+  iApply isim_yield;
+  iSplitL hyps; [ |iIntros "% % % % %"; iIntrosFresh "IST"].
+
+Lemma isim_apc_tgt_remove `{Σ: GRA.t}
+  fl fr Ist r g {R} RR my_tid ps pt nths st_src st_tgt i_src k_tgt scopes stb
+  :
+  bi_entails
+    (@isim Σ fl fr Ist my_tid r g R RR ps true nths (st_src, i_src) (st_tgt, k_tgt tt))
+    (isim fl fr Ist my_tid r g RR ps pt nths (st_src, i_src) (st_tgt,
+         HModSem.sandbox scopes (HoareAPC stb (ord_pure Ord.O)) >>= k_tgt)).
+Proof.
+  iIntros "ISIM". unfold HoareAPC.
+  steps_r. rewrite unfold_APC. steps_r.
+  des_ifs.
+  - steps_r; eauto.
+  - steps_r. hss.
+    iDestruct "GRT" as "(_ & % & _)".
+    exfalso. destruct (q7 q4).
+    + rr in H. assert (X := Ord.O_bot n).
+      eapply Ord.lt_not_le; eauto.
+    + rr in H. eauto.
+Qed.
+
+Ltac apc_l :=
+  rewrite/__ {1}/HoareAPC; force_l; instantiate (1:= Ord.O);
+  rewrite unfold_APC; force_l; instantiate (1:=true); step_l.
+
+Ltac apc_r :=
+  hide_itree_l;
+  prep;
+  match goal with
+  | [ |- environments.envs_entails _ (isim _ _ _ _ _ _ _ _ _ _ _ (_, (HModSem.sandbox _ (HoareAPC _ _)) >>= _)) ] =>
+      iApply isim_apc_tgt_remove
+  end;
+  show_itree.
+
+Ltac init_simF :=
+  unfold HSim.sim_fun, HSSim.sim_fun; i;
+  match goal with [H: _|-_] => revert H end;
+  s; unfold_hmod;
+  match goal with [|-context[alist_find _ ?x]] =>
+    set (TMP := x); unfold_hmod; unfold TMP; clear TMP
+  end;
+  simpl HModSem.fnsems;
+  alist_find_simpl fnsems_nodup;
+  let H := fresh "TMP" in intros H; inv H;
+  alist_find_simpl fnsems_nodup;
+  eexists; split; [eauto|];
+  repeat match goal with
+  | [|- context[{| fsb_body := cfunU ?x |}]] => rewrite/__ {1}/x
+  | [|- context[{| fsb_body := ?x |}]] => rewrite/__ {1}/x
+  | [|- context[cfunU ?x]] => rewrite/__ {1}/x
+  end;                          
+  unfold interp_sb_hp, HoareFun, cfunU, ccallU, HModSem.sandbox_body; s;
+  ii; subst; iIntros "IST".
+
+Ltac prove_sub_perm :=
+  i; try rewrite /HMod.scopes; s; repeat unfold_hmod; s; Lauto_normalize;
+  match goal with
+    [|-sub_perm ?x ?y] =>
+      match x with
+      | _ ++ _ => idtac
+      | _ => rewrite/__ /x
+      end;
+      match y with
+      | _ ++ _ => idtac
+      | _ => rewrite/__ /y
+      end
+  end;
+  Lauto_normalize;
+  match goal with
+    [|-sub_perm ?x ?y] =>
+      replace (sub_perm x y) with (sub_perm (x++[]) (y++[])) by (rewrite !app_nil_r; eauto)
+  end;
+  repeat first [eapply sub_perm_cancel_head|eapply sub_perm_remove_head];
+  eapply sub_perm_refl.
+
+(**** TODO ****)
+(* A tactic to handle meta variables *)
+(* Tactics to handle APC. (APC in src / in tgt / ord_pure 0 / ord_pure n / ....  ) *)
+
+(************ User Notations **************)
+
+From iris.proofmode Require Import coq_tactics environments.
+
+Global Arguments Envs _ _%proof_scope _%proof_scope _.
+Global Arguments Enil {_}.
+Global Arguments Esnoc {_} _%proof_scope _%string _%I.
+
+Local Notation world_id := positive.
+Local Notation level := nat.
+
+(*** TODO: 
+          What else should be displayed? 
+          Simplify (hide) k-trees
+
+***)
+
+(*** isim ***)
+Notation "E1 '------------------------------------------------------------------□' E2 '------------------------------------------------------------------∗' st_src st_tgt '-------------------------------isim-------------------------------'  itr_src itr_tgt"
+:=
+  (environments.envs_entails (Envs E1 E2 _) (isim _ _ _ _ _ _ _ _ _ _ (st_src, itr_src) (st_tgt, itr_tgt)))
+    (at level 50,
+     format "E1 '------------------------------------------------------------------□' '//' E2 '------------------------------------------------------------------∗' '//' st_src '//' st_tgt '//' '-------------------------------isim-------------------------------' '//' itr_src '//' '//' '//' itr_tgt '//' ").
+
+Notation "E1 '------------------------------------------------------------------□' st_src st_tgt '-------------------------------isim-------------------------------'  itr_src itr_tgt"
+:=
+  (environments.envs_entails (Envs E1 Enil _) (isim _ _ _ _ _ _ _ _ _ _ (st_src, itr_src) (st_tgt, itr_tgt)))
+    (at level 50,
+     format "E1 '------------------------------------------------------------------□' '//' st_src '//' st_tgt '//' '-------------------------------isim-------------------------------' '//' itr_src '//' '//' '//' itr_tgt '//' ").
+
+Notation "E2 '------------------------------------------------------------------∗' st_src st_tgt '-------------------------------isim-------------------------------'  itr_src itr_tgt"
+:=
+  (environments.envs_entails (Envs Enil E2 _) (isim _ _ _ _ _ _ _ _ _ _ (st_src, itr_src) (st_tgt, itr_tgt)))
+    (at level 50,
+     format "E2 '------------------------------------------------------------------∗' '//' st_src '//' st_tgt '//' '-------------------------------isim-------------------------------' '//' itr_src '//' '//' '//' itr_tgt '//' ").
+
+Notation "'------------------------------------------------------------------∗' st_src st_tgt '-------------------------------isim-------------------------------'  itr_src itr_tgt"
+:=
+  (environments.envs_entails (Envs Enil Enil _) (isim _ _ _ _ _ _ _ _ _ _ (st_src, itr_src) (st_tgt, itr_tgt)))
+    (at level 50,
+     format "'------------------------------------------------------------------∗' '//' st_src '//' st_tgt '//' '-------------------------------isim-------------------------------' '//' itr_src '//' '//' '//' itr_tgt '//' ").
+
+(* additional *) 
+Notation "E1 '------------------------------------------------------------------□' E2 '------------------------------------------------------------------∗' st_src st_tgt '-------------------------------isim-------------------------------'  P '∗' 'ISIM'"
+:=
+  (environments.envs_entails (Envs E1 E2 _) (bi_sep P (isim _ _ _ _ _ _ _ _ _ _ (st_src, _) (st_tgt, _))))
+    (at level 50,
+     format "E1 '------------------------------------------------------------------□' '//' E2 '------------------------------------------------------------------∗' '//' st_src '//' st_tgt '//' '-------------------------------isim-------------------------------' '//' P  '∗'  'ISIM' ").
+
+Notation "E1 '------------------------------------------------------------------□' E2 '------------------------------------------------------------------∗' st_src st_tgt '-------------------------------isim-------------------------------'  P '-∗' 'ISIM'"
+:=
+  (environments.envs_entails (Envs E1 E2 _) (bi_wand P (isim _ _ _ _ _ _ _ _ _ _ (st_src, _) (st_tgt, _))))
+    (at level 50,
+     format "E1 '------------------------------------------------------------------□' '//' E2 '------------------------------------------------------------------∗' '//' st_src '//' st_tgt '//' '-------------------------------isim-------------------------------' '//' P  '-∗'  'ISIM' ").
+
+
